LottExamples/SystemF.lean
@@ -1,10 +1,15 @@
 import Lott
+import Lott.Data.List
+import Lott.DSL.Elab.UniversalJudgement
 
 namespace LottExamples.SystemF
 
 open Lean
 
+locally_nameless
 metavar TypeVar, a, b
+
+locally_nameless
 metavar TermVar, x, y
 
 nonterminal Type', A, B :=
@@ -13,28 +18,202 @@ nonterminal Type', A, B :=
   | "∀ " a ". " A        : forall' (bind a in A)
   | "(" A ")"            : paren (desugar := return A)
 
-theorem Type'.forall_subst_eq_subst_forall (aneb : a ≠ b)
-  : [[∀ a. (A [B / b])]] = [[(∀ a. A) [B / b] ]] := by rw [Type'.TypeVar_subst, if_neg aneb.symm]
-
-theorem Type'.subst_subst : [[(A' [A / a] [B / a])]] = [[(A' [A [B / a] / a])]] := by
-  match A' with
-  | .var a' =>
-    rw [Type'.TypeVar_subst, Type'.TypeVar_subst]
+@[simp]
+theorem Type'.TypeVar_open_sizeOf (A : Type') : sizeOf (A.TypeVar_open a n) = sizeOf A := by
+  match A with
+  | var (.bound _) =>
+    rw [TypeVar_open]
     split
-    · case isTrue a'eqa => rfl
-    · case isFalse a'nea => rw [Type'.TypeVar_subst, if_neg a'nea]
-  | .arr A' B' =>
-    rw [Type'.TypeVar_subst, Type'.TypeVar_subst]
-    rw [Type'.subst_subst, Type'.subst_subst]
-    rw [← Type'.TypeVar_subst]
-  | .forall' a' A' =>
-    rw [Type'.TypeVar_subst, Type'.TypeVar_subst]
+    · case isTrue h' =>
+      dsimp only [sizeOf]
+      rw [← h', _sizeOf_1, _sizeOf_1]
+      dsimp only [sizeOf]
+      rw [default.sizeOf, default.sizeOf]
+    · case isFalse => rfl
+  | var (.free _) =>
+    rw [TypeVar_open]
     split
-    · case isTrue a'eqa => rw [Type'.TypeVar_subst, if_pos a'eqa]
-    · case isFalse a'nea => rw [Type'.TypeVar_subst, Type'.subst_subst, if_neg a'nea]
+    · case isTrue => rw [if_neg id]
+    · case isFalse => rfl
+  | arr A' B =>
+    dsimp only [sizeOf]
+    rw [TypeVar_open, _sizeOf_1, _sizeOf_1]
+    simp only
+    rw [← _sizeOf_1, ← _sizeOf_1, ← _sizeOf_1, ← _sizeOf_1]
+    have : ∀ a : Type', a._sizeOf_1 = sizeOf a := fun _ => by dsimp only [sizeOf]
+    rw [this (A'.TypeVar_open _ _), this (B.TypeVar_open _ _), this A', this B]
+    rw [A'.TypeVar_open_sizeOf, B.TypeVar_open_sizeOf]
+  | forall' A' =>
+    dsimp only [sizeOf]
+    rw [TypeVar_open, _sizeOf_1, _sizeOf_1]
+    simp only
+    rw [← _sizeOf_1, ← _sizeOf_1]
+    have : ∀ a : Type', a._sizeOf_1 = sizeOf a := fun _ => by dsimp only [sizeOf]
+    rw [this (A'.TypeVar_open _ _), this A', A'.TypeVar_open_sizeOf]
 
-theorem Type'.subst_shadowed_forall (B : Type') : [[∀ a. A]] = [[(∀ a. A) [B / a] ]] := by
-  rw [Type'.TypeVar_subst, if_pos rfl]
+theorem Type'.TypeVar_open_comm (A : Type') (anea' : a ≠ a') (mnen : m ≠ n)
+  : (A.TypeVar_open a m).TypeVar_open a' n =
+    (A.TypeVar_open a' n).TypeVar_open a m := by match A with
+  | var (.free _) =>
+    rw [TypeVar_open, if_neg (nomatch ·), TypeVar_open, if_neg (nomatch ·), TypeVar_open,
+        if_neg (nomatch ·)]
+  | var (.bound _) =>
+    rw [TypeVar_open]
+    split
+    · case isTrue h =>
+      rw [← h, TypeVar_open, if_neg (nomatch ·), TypeVar_open,
+          if_neg (mnen <| TypeVar.bound.inj ·.symm), TypeVar_open, if_pos rfl]
+    · case isFalse h =>
+      rw [TypeVar_open]
+      split
+      · case isTrue h' => rw [TypeVar_open, if_neg (nomatch ·)]
+      · case isFalse h' => rw [TypeVar_open, if_neg h]
+  | arr A' B =>
+    rw [TypeVar_open, TypeVar_open, A'.TypeVar_open_comm anea' mnen, B.TypeVar_open_comm anea' mnen,
+        ← TypeVar_open, ← TypeVar_open]
+  | forall' A' =>
+    rw [TypeVar_open, TypeVar_open]
+    simp only
+    rw [A'.TypeVar_open_comm anea' (mnen <| Nat.succ_inj'.mp ·), ← TypeVar_open, ← TypeVar_open]
+
+inductive Type'.TypeVarLocallyClosed : Type' → Nat → Prop where
+  | var_free : TypeVarLocallyClosed (.var (.free _)) n
+  | var_bound : m < n → TypeVarLocallyClosed (.var (.bound m)) n
+  | arr {A B : Type'}
+    : A.TypeVarLocallyClosed n → B.TypeVarLocallyClosed n → (A.arr B).TypeVarLocallyClosed n
+  | forall' {A : Type'} : A.TypeVarLocallyClosed (n + 1) → A.forall'.TypeVarLocallyClosed n
+
+theorem Type'.TypeVarLocallyClosed.weaken {A : Type'}
+  : A.TypeVarLocallyClosed m → A.TypeVarLocallyClosed (m + n)
+  | var_free => var_free
+  | var_bound h => var_bound <| Nat.lt_add_right _ h
+  | arr A'lc Blc => arr A'lc.weaken Blc.weaken
+  | forall' A'lc => by
+    apply forall'
+    rw [Nat.add_assoc, Nat.add_comm _ 1, ← Nat.add_assoc]
+    exact A'lc.weaken
+
+theorem Type'.TypeVarLocallyClosed.TypeVar_open_drop {A : Type'} (h : m < n)
+  : (A.TypeVar_open a m).TypeVarLocallyClosed n → A.TypeVarLocallyClosed n := fun Alc => by
+  match A with
+  | .var _ =>
+    rw [TypeVar_open] at Alc
+    split at Alc
+    · case isTrue h' =>
+      rw [← h']
+      exact var_bound h
+    · case isFalse h' => exact Alc
+  | .arr A' B =>
+    rw [TypeVar_open] at Alc
+    let .arr A'lc Blc := Alc
+    exact arr (A'lc.TypeVar_open_drop h) (Blc.TypeVar_open_drop h)
+  | .forall' A' =>
+    rw [TypeVar_open] at Alc
+    let .forall' A'lc := Alc
+    exact forall' <| A'lc.TypeVar_open_drop <| Nat.add_lt_add_iff_right.mpr h
+
+theorem Type'.TypeVarLocallyClosed.TypeVar_open_eq {A : Type'}
+  (h : A.TypeVarLocallyClosed m) (mlen : m ≤ n)
+  : A.TypeVar_open x n = A := by match A, h with
+  | var (.free _), var_free => rw [TypeVar_open, if_neg (nomatch ·)]
+  | var (.bound _), var_bound lt =>
+    have := Nat.ne_of_lt <| Nat.lt_of_lt_of_le lt mlen
+    rw [TypeVar_open, if_neg fun x => this.symm <| TypeVar.bound.inj x]
+  | .arr A' B, arr A'lc Blc =>
+    rw [TypeVar_open, A'lc.TypeVar_open_eq mlen, Blc.TypeVar_open_eq mlen]
+  | .forall' A, forall' A'lc =>
+    rw [TypeVar_open]
+    simp only
+    rw [A'lc.TypeVar_open_eq (Nat.add_le_add_iff_right.mpr mlen)]
+
+theorem Type'.TypeVarLocallyClosed.Type'_open_eq {A : Type'}
+  (h : A.TypeVarLocallyClosed m) (mlen : m ≤ n)
+  : A.Type'_open B n = A := by match A, h with
+  | var (.free _), var_free => rw [Type'_open, if_neg (nomatch ·)]
+  | var (.bound _), var_bound lt =>
+    have := Nat.ne_of_lt <| Nat.lt_of_lt_of_le lt mlen
+    rw [Type'_open, if_neg fun x => this.symm <| TypeVar.bound.inj x]
+  | .arr A' B, arr A'lc Blc =>
+    rw [Type'_open, A'lc.Type'_open_eq mlen, Blc.Type'_open_eq mlen]
+  | .forall' A, forall' A'lc =>
+    rw [Type'_open]
+    simp only
+    rw [A'lc.Type'_open_eq (Nat.add_le_add_iff_right.mpr mlen)]
+
+theorem Type'.Type'_open_comm (A : Type') {B A': Type'} (mnen : m ≠ n)
+  (Blc : B.TypeVarLocallyClosed n) (A'lc : A'.TypeVarLocallyClosed m)
+  : (A.Type'_open B m).Type'_open A' n =
+    (A.Type'_open A' n).Type'_open B m := by match A with
+  | var (.free _) =>
+    rw [Type'_open, if_neg (nomatch ·), Type'_open, if_neg (nomatch ·), Type'_open,
+        if_neg (nomatch ·)]
+  | var (.bound _) =>
+    rw [Type'_open]
+    split
+    · case isTrue h =>
+      rw [← h, Blc.Type'_open_eq (Nat.le_refl _), Type'_open,
+          if_neg (mnen <| TypeVar.bound.inj ·.symm), Type'_open, if_pos rfl]
+    · case isFalse h =>
+      rw [Type'_open]
+      split
+      · case isTrue h' => rw [A'lc.Type'_open_eq (Nat.le_refl _)]
+      · case isFalse h' => rw [Type'_open, if_neg h]
+  | arr A' B =>
+    rw [Type'_open, Type'_open, A'.Type'_open_comm mnen Blc A'lc, B.Type'_open_comm mnen Blc A'lc,
+        ← Type'_open, ← Type'_open]
+  | forall' A' =>
+    rw [Type'_open, Type'_open]
+    simp only
+    rw [A'.Type'_open_comm (mnen <| Nat.succ_inj'.mp ·) (Blc.weaken (n := 1))
+          (A'lc.weaken (n := 1)), ← Type'_open, ← Type'_open]
+
+theorem Type'.TypeVar_open_Type'_open_eq {A B : Type'}
+  (Blc : B.TypeVarLocallyClosed m) (mnen : m ≠ n)
+  : (A.TypeVar_open a m).Type'_open B n =
+    (A.Type'_open B n).TypeVar_open a m := by
+  match A with
+  | var (.free _) =>
+    rw [TypeVar_open, if_neg (nomatch ·), Type'_open, if_neg (nomatch ·), TypeVar_open,
+        if_neg (nomatch ·)]
+  | var (.bound _) =>
+    rw [TypeVar_open]
+    split
+    · case isTrue h =>
+      rw [Type'_open, if_neg (nomatch ·), Type'_open, ← h,
+          if_neg (mnen <| TypeVar.bound.inj ·.symm), TypeVar_open, if_pos rfl]
+    · case isFalse h =>
+      rw [Type'_open]
+      split
+      · case isTrue h' => rw [Blc.TypeVar_open_eq (Nat.le_refl _)]
+      · case isFalse h' => rw [TypeVar_open, if_neg h]
+  | arr A' B' =>
+    rw [TypeVar_open, Type'_open, TypeVar_open_Type'_open_eq Blc mnen,
+        TypeVar_open_Type'_open_eq Blc mnen, ← TypeVar_open, ← Type'_open]
+  | forall' A' =>
+    rw [TypeVar_open, Type'_open]
+    simp only
+    rw [TypeVar_open_Type'_open_eq Blc.weaken
+          (by exact mnen <| Nat.succ_inj'.mp ·), ← TypeVar_open, ← Type'_open]
+
+theorem Type'.TypeVar_open_Type'_open_eq' {A B : Type'}
+  (Blc : B.TypeVarLocallyClosed n)
+  : (A.TypeVar_open a n).Type'_open B n =
+    A.TypeVar_open a n := by
+  match A with
+  | var (.free _) =>
+    rw [TypeVar_open, if_neg (nomatch ·), Type'_open, if_neg (nomatch ·)]
+  | var (.bound _) =>
+    rw [TypeVar_open]
+    split
+    · case isTrue h => rw [Type'_open, if_neg (nomatch ·)]
+    · case isFalse h => rw [Type'_open, if_neg h]
+  | arr A' B' =>
+    rw [TypeVar_open, Type'_open, TypeVar_open_Type'_open_eq' Blc, TypeVar_open_Type'_open_eq' Blc,
+        ← TypeVar_open]
+  | forall' A' =>
+    rw [TypeVar_open, Type'_open]
+    simp only
+    rw [TypeVar_open_Type'_open_eq' Blc.weaken, ← TypeVar_open]
 
 nonterminal Term, E, F :=
   | x                     : var
@@ -44,55 +223,542 @@ nonterminal Term, E, F :=
   | E " [" A "]"          : typeApp
   | "(" E ")"             : paren (desugar := return E)
 
+@[simp]
+theorem Term.TermVar_open_sizeOf (E : Term) : sizeOf (E.TermVar_open x n) = sizeOf E := by
+  match E with
+  | var (.bound _) =>
+    rw [TermVar_open]
+    split
+    · case isTrue h' =>
+      dsimp only [sizeOf]
+      rw [← h', _sizeOf_1, _sizeOf_1]
+      dsimp only [sizeOf]
+      rw [default.sizeOf, default.sizeOf]
+    · case isFalse => rfl
+  | var (.free _) =>
+    rw [TermVar_open]
+    split
+    · case isTrue => rw [if_neg id]
+    · case isFalse => rfl
+  | lam A E' =>
+    dsimp [sizeOf]
+    rw [TermVar_open, _sizeOf_1, _sizeOf_1]
+    simp only
+    rw [← _sizeOf_1, ← _sizeOf_1]
+    have : ∀ a : Term, a._sizeOf_1 = sizeOf a := fun _ => by dsimp only [sizeOf]
+    rw [this _, this _]
+    have : ∀ a : Type', a._sizeOf_1 = sizeOf a := fun _ => by dsimp only [sizeOf]
+    rw [this _, E'.TermVar_open_sizeOf]
+  | app E' F =>
+    dsimp [sizeOf]
+    rw [TermVar_open, _sizeOf_1, _sizeOf_1]
+    simp only
+    rw [← _sizeOf_1, ← _sizeOf_1, ← _sizeOf_1]
+    have : ∀ a : Term, a._sizeOf_1 = sizeOf a := fun _ => by dsimp only [sizeOf]
+    rw [this _, this _, this _, this _, E'.TermVar_open_sizeOf,
+        F.TermVar_open_sizeOf]
+  | typeGen E' =>
+    dsimp [sizeOf]
+    rw [TermVar_open, _sizeOf_1, _sizeOf_1]
+    simp only
+    rw [← _sizeOf_1, ← _sizeOf_1]
+    have : ∀ a : Term, a._sizeOf_1 = sizeOf a := fun _ => by dsimp only [sizeOf]
+    rw [this _, this _, E'.TermVar_open_sizeOf]
+  | typeApp E' A =>
+    dsimp [sizeOf]
+    rw [TermVar_open, _sizeOf_1, _sizeOf_1]
+    simp only
+    rw [← _sizeOf_1, ← _sizeOf_1]
+    have : ∀ a : Term, a._sizeOf_1 = sizeOf a := fun _ => by dsimp only [sizeOf]
+    rw [this _, this _]
+    have : ∀ a : Type', a._sizeOf_1 = sizeOf a := fun _ => by dsimp only [sizeOf]
+    rw [this _, E'.TermVar_open_sizeOf]
+
+@[simp]
+theorem Term.TypeVar_open_sizeOf (E : Term) : sizeOf (E.TypeVar_open x n) = sizeOf E := by
+  match E with
+  | var _ => rw [TypeVar_open]
+  | lam A E' =>
+    dsimp [sizeOf]
+    rw [TypeVar_open, _sizeOf_1, _sizeOf_1]
+    simp only
+    rw [← _sizeOf_1, ← _sizeOf_1]
+    have : ∀ a : Term, a._sizeOf_1 = sizeOf a := fun _ => by dsimp only [sizeOf]
+    rw [this _, this _]
+    have : ∀ a : Type', a._sizeOf_1 = sizeOf a := fun _ => by dsimp only [sizeOf]
+    rw [this _, A.TypeVar_open_sizeOf, E'.TypeVar_open_sizeOf]
+  | app E' F =>
+    dsimp [sizeOf]
+    rw [TypeVar_open, _sizeOf_1, _sizeOf_1]
+    simp only
+    rw [← _sizeOf_1, ← _sizeOf_1, ← _sizeOf_1]
+    have : ∀ a : Term, a._sizeOf_1 = sizeOf a := fun _ => by dsimp only [sizeOf]
+    rw [this _, this _, this _, this _, E'.TypeVar_open_sizeOf, F.TypeVar_open_sizeOf]
+  | typeGen E' =>
+    dsimp [sizeOf]
+    rw [TypeVar_open, _sizeOf_1, _sizeOf_1]
+    simp only
+    rw [← _sizeOf_1, ← _sizeOf_1]
+    have : ∀ a : Term, a._sizeOf_1 = sizeOf a := fun _ => by dsimp only [sizeOf]
+    rw [this _, this _, E'.TypeVar_open_sizeOf]
+  | typeApp E' A =>
+    dsimp [sizeOf]
+    rw [TypeVar_open, _sizeOf_1, _sizeOf_1]
+    simp only
+    rw [← _sizeOf_1, ← _sizeOf_1]
+    have : ∀ a : Term, a._sizeOf_1 = sizeOf a := fun _ => by dsimp only [sizeOf]
+    rw [this _, this _]
+    have : ∀ a : Type', a._sizeOf_1 = sizeOf a := fun _ => by dsimp only [sizeOf]
+    rw [this _, E'.TypeVar_open_sizeOf, A.TypeVar_open_sizeOf]
+
+theorem Term.TermVar_open_comm (E : Term) (xnex' : x ≠ x') (mnen : m ≠ n)
+  : (E.TermVar_open x m).TermVar_open x' n =
+    (E.TermVar_open x' n).TermVar_open x m := by match E with
+  | var (.free _) =>
+    rw [TermVar_open, if_neg (nomatch ·), TermVar_open, if_neg (nomatch ·), TermVar_open,
+        if_neg (nomatch ·)]
+  | var (.bound _) =>
+    rw [TermVar_open]
+    split
+    · case isTrue h =>
+      rw [← h, TermVar_open, if_neg (nomatch ·), TermVar_open,
+          if_neg (mnen <| TermVar.bound.inj ·.symm), TermVar_open, if_pos rfl]
+    · case isFalse h =>
+      rw [TermVar_open]
+      split
+      · case isTrue h' => rw [TermVar_open, if_neg (nomatch ·)]
+      · case isFalse h' => rw [TermVar_open, if_neg h]
+  | lam A E' =>
+    rw [TermVar_open, TermVar_open]
+    simp only
+    rw [E'.TermVar_open_comm xnex' (mnen <| Nat.succ_inj'.mp ·), ← TermVar_open, ← TermVar_open]
+  | app E' F =>
+    rw [TermVar_open, TermVar_open, E'.TermVar_open_comm xnex' mnen, F.TermVar_open_comm xnex' mnen,
+        ← TermVar_open, ← TermVar_open]
+  | typeGen E' =>
+    rw [TermVar_open, TermVar_open, E'.TermVar_open_comm xnex' mnen, ← TermVar_open, ← TermVar_open]
+  | typeApp E' A =>
+    rw [TermVar_open, TermVar_open, E'.TermVar_open_comm xnex' mnen, ← TermVar_open, ← TermVar_open]
+
+theorem Term.TypeVar_open_comm (E : Term) (anea' : a ≠ a') (mnen : m ≠ n)
+  : (E.TypeVar_open a m).TypeVar_open a' n =
+    (E.TypeVar_open a' n).TypeVar_open a m := by match E with
+  | var _ => rw [TypeVar_open, TypeVar_open, TypeVar_open]
+  | lam A E' =>
+    rw [TypeVar_open, TypeVar_open, A.TypeVar_open_comm anea' mnen, E'.TypeVar_open_comm anea' mnen,
+        ← TypeVar_open, ← TypeVar_open]
+  | app E' F =>
+    rw [TypeVar_open, TypeVar_open, E'.TypeVar_open_comm anea' mnen, F.TypeVar_open_comm anea' mnen,
+        ← TypeVar_open, ← TypeVar_open]
+  | typeGen E' =>
+    rw [TypeVar_open, TypeVar_open]
+    simp only
+    rw [E'.TypeVar_open_comm anea' (mnen <| Nat.succ_inj'.mp ·), ← TypeVar_open, ← TypeVar_open]
+  | typeApp E' A =>
+    rw [TypeVar_open, TypeVar_open, E'.TypeVar_open_comm anea' mnen, A.TypeVar_open_comm anea' mnen,
+        ← TypeVar_open, ← TypeVar_open]
+
+theorem Term.TermVar_open_Type'_open_comm (E : Term)
+  : (E.TermVar_open x m).Type'_open A n = (E.Type'_open A n).TermVar_open x m := by match E with
+  | var _ =>
+    rw [TermVar_open]
+    split
+    · case isTrue h => rw [Type'_open, Type'_open, TermVar_open, if_pos h]
+    · case isFalse h => rw [Type'_open, TermVar_open, if_neg h]
+  | lam A' E' =>
+     rw [TermVar_open, Type'_open, E'.TermVar_open_Type'_open_comm, ← TermVar_open, ← Type'_open]
+  | app E' F =>
+    rw [TermVar_open, Type'_open, E'.TermVar_open_Type'_open_comm, F.TermVar_open_Type'_open_comm,
+        ← TermVar_open, ← Type'_open]
+  | typeGen E' =>
+    rw [TermVar_open, Type'_open]
+    simp only
+    rw [E'.TermVar_open_Type'_open_comm, ← TermVar_open, ← Type'_open]
+  | typeApp E' A' =>
+    rw [TermVar_open, Type'_open, E'.TermVar_open_Type'_open_comm, ← TermVar_open, ← Type'_open]
+
+inductive Term.TermVarLocallyClosed : Term → Nat → Prop where
+  | var_free : TermVarLocallyClosed (var (.free _)) n
+  | var_bound : m < n → TermVarLocallyClosed (var (.bound m)) n
+  | lam : E.TermVarLocallyClosed (n + 1) → (lam A E).TermVarLocallyClosed n
+  | app {E F : Term}
+    : E.TermVarLocallyClosed n → F.TermVarLocallyClosed n → (E.app F).TermVarLocallyClosed n
+  | typeGen {E : Term} : E.TermVarLocallyClosed n → E.typeGen.TermVarLocallyClosed n
+  | typeApp {E : Term} : E.TermVarLocallyClosed n → (E.typeApp A).TermVarLocallyClosed n
+
+theorem Term.TermVarLocallyClosed.weaken {E : Term}
+  : E.TermVarLocallyClosed m → E.TermVarLocallyClosed (m + n)
+  | var_free => var_free
+  | var_bound h => var_bound <| Nat.lt_add_right _ h
+  | lam E'lc => by
+    apply lam
+    rw [Nat.add_assoc, Nat.add_comm _ 1, ← Nat.add_assoc]
+    exact E'lc.weaken
+  | app E'lc Flc => app E'lc.weaken Flc.weaken
+  | typeGen E'lc => typeGen E'lc.weaken
+  | typeApp E'lc => typeApp E'lc.weaken
+
+theorem Term.TermVarLocallyClosed.TermVar_open_drop {E : Term} (h : m < n)
+  : (E.TermVar_open x m).TermVarLocallyClosed n → E.TermVarLocallyClosed n := fun Elc => by
+  match E with
+  | .var _ =>
+    rw [TermVar_open] at Elc
+    split at Elc
+    · case isTrue h' =>
+      rw [← h']
+      exact var_bound h
+    · case isFalse h' => exact Elc
+  | .lam _ E' =>
+    rw [TermVar_open] at Elc
+    let .lam E'lc := Elc
+    exact lam <| E'lc.TermVar_open_drop <| Nat.add_lt_add_iff_right.mpr h
+  | .app E' F =>
+    rw [TermVar_open] at Elc
+    let .app E'lc Flc := Elc
+    exact app (E'lc.TermVar_open_drop h) (Flc.TermVar_open_drop h)
+  | .typeGen E' =>
+    rw [TermVar_open] at Elc
+    let .typeGen E'lc := Elc
+    exact typeGen <| E'lc.TermVar_open_drop h
+  | .typeApp E' A =>
+    rw [TermVar_open] at Elc
+    let .typeApp E'lc := Elc
+    exact typeApp <| E'lc.TermVar_open_drop h
+
+theorem Term.TermVarLocallyClosed.TypeVar_open_drop {E : Term}
+  : (E.TypeVar_open a m).TermVarLocallyClosed n → E.TermVarLocallyClosed n := fun Elc => by
+  match E with
+  | .var _ =>
+    rw [TypeVar_open] at Elc
+    exact Elc
+  | .lam _ E' =>
+    rw [TypeVar_open] at Elc
+    let .lam E'lc := Elc
+    exact lam E'lc.TypeVar_open_drop
+  | .app E' F =>
+    rw [TypeVar_open] at Elc
+    let .app E'lc Flc := Elc
+    exact app E'lc.TypeVar_open_drop Flc.TypeVar_open_drop
+  | .typeGen E' =>
+    rw [TypeVar_open] at Elc
+    let .typeGen E'lc := Elc
+    exact typeGen E'lc.TypeVar_open_drop
+  | .typeApp E' A =>
+    rw [TypeVar_open] at Elc
+    let .typeApp E'lc := Elc
+    exact typeApp E'lc.TypeVar_open_drop
+
+theorem Term.TermVarLocallyClosed.TermVar_open_eq {E : Term} (h : E.TermVarLocallyClosed m)
+  (mlen : m ≤ n) : E.TermVar_open x n = E := by match E, h with
+  | var (.free _), var_free => rw [TermVar_open, if_neg (nomatch ·)]
+  | var (.bound _), var_bound lt =>
+    have := Nat.ne_of_lt <| Nat.lt_of_lt_of_le lt mlen
+    rw [TermVar_open, if_neg fun x => this.symm <| TermVar.bound.inj x]
+  | .lam A E', lam E'lc =>
+    rw [TermVar_open]
+    simp only
+    rw [E'lc.TermVar_open_eq (Nat.add_le_add_iff_right.mpr mlen)]
+  | .app E' F, app E'lc Flc =>
+    rw [TermVar_open, E'lc.TermVar_open_eq mlen, Flc.TermVar_open_eq mlen]
+  | .typeGen E', typeGen E'lc => rw [TermVar_open, E'lc.TermVar_open_eq mlen]
+  | .typeApp E' A, typeApp E'lc => rw [TermVar_open, E'lc.TermVar_open_eq mlen]
+
+theorem Term.TermVar_open_TermVar_subst_eq {E F : Term} (xnex' : x ≠ x')
+  (Flc : F.TermVarLocallyClosed n)
+  : (E.TermVar_open x n).TermVar_subst x' F = (E.TermVar_subst x' F).TermVar_open x n := by
+  match E with
+  | var x'' =>
+    rw [TermVar_open, TermVar_subst, TermVar_subst]
+    split
+    · case isTrue h =>
+      rw [← h, if_neg fun x => xnex' <| TermVar.free.inj x.symm, if_neg (nomatch ·), TermVar_open,
+          if_pos rfl]
+    · case isFalse h =>
+      split
+      · case isTrue h' => rw [Flc.TermVar_open_eq (Nat.le_refl _)]
+      · case isFalse h' => rw [TermVar_open, if_neg h]
+  | lam A E' =>
+    rw [TermVar_open, TermVar_subst, TermVar_subst, TermVar_open,
+        E'.TermVar_open_TermVar_subst_eq xnex' Flc.weaken]
+  | app E' F =>
+    rw [TermVar_open, TermVar_subst, TermVar_subst, TermVar_open,
+        E'.TermVar_open_TermVar_subst_eq xnex' Flc,
+        F.TermVar_open_TermVar_subst_eq xnex' Flc]
+  | typeGen E' =>
+    rw [TermVar_open, TermVar_subst, TermVar_subst, TermVar_open,
+        E'.TermVar_open_TermVar_subst_eq xnex' Flc]
+  | typeApp E' A =>
+    rw [TermVar_open, TermVar_subst, TermVar_subst, TermVar_open,
+        E'.TermVar_open_TermVar_subst_eq xnex' Flc]
+
+theorem Term.TermVar_open_Term_open_eq {E F : Term}
+  (Flc : F.TermVarLocallyClosed m) (mnen : m ≠ n)
+  : (E.TermVar_open x m).Term_open F n =
+    (E.Term_open F n).TermVar_open x m := by
+  match E with
+  | var (.free _) =>
+    rw [TermVar_open, if_neg (nomatch ·), Term_open, if_neg (nomatch ·), TermVar_open,
+        if_neg (nomatch ·)]
+  | var (.bound _) =>
+    rw [TermVar_open]
+    split
+    · case isTrue h =>
+      rw [Term_open, if_neg (nomatch ·), Term_open, ← h, if_neg (mnen <| TermVar.bound.inj ·.symm),
+          TermVar_open, if_pos rfl]
+    · case isFalse h =>
+      rw [Term_open]
+      split
+      · case isTrue h' => rw [Flc.TermVar_open_eq (Nat.le_refl _)]
+      · case isFalse h' => rw [TermVar_open, if_neg h]
+  | lam A E' =>
+    rw [TermVar_open, Term_open]
+    simp only
+    rw [TermVar_open_Term_open_eq Flc.weaken (by exact mnen <| Nat.succ_inj'.mp ·), ← TermVar_open,
+        ← Term_open]
+  | app E' F =>
+    rw [TermVar_open, Term_open, TermVar_open_Term_open_eq Flc mnen,
+        TermVar_open_Term_open_eq Flc mnen, ← TermVar_open, ← Term_open]
+  | typeGen E' =>
+    rw [TermVar_open, Term_open, TermVar_open_Term_open_eq Flc mnen, ← TermVar_open, ← Term_open]
+  | typeApp E' A =>
+    rw [TermVar_open, Term_open, TermVar_open_Term_open_eq Flc mnen, ← TermVar_open, ← Term_open]
+
+theorem Term.TermVar_open_TypeVar_open_eq (E : Term)
+  : (E.TermVar_open x m).TypeVar_open a n =
+    (E.TypeVar_open a n).TermVar_open x m := by match E with
+  | var (.free _) =>
+    rw [TermVar_open, if_neg (nomatch ·), TypeVar_open, TermVar_open, if_neg (nomatch ·)]
+  | var (.bound _) =>
+    rw [TermVar_open]
+    split
+    · case isTrue h => rw [← h, TypeVar_open, TypeVar_open, TermVar_open, if_pos rfl]
+    · case isFalse h => rw [TypeVar_open, TermVar_open, if_neg h]
+  | lam A E' =>
+    rw [TermVar_open, TypeVar_open, TermVar_open_TypeVar_open_eq, ← TermVar_open, ← TypeVar_open]
+  | app E' F =>
+    rw [TermVar_open, TypeVar_open, TermVar_open_TypeVar_open_eq, TermVar_open_TypeVar_open_eq,
+        ← TermVar_open, ← TypeVar_open]
+  | typeGen E' =>
+    rw [TermVar_open, TypeVar_open]
+    simp only
+    rw [TermVar_open_TypeVar_open_eq, ← TermVar_open, ← TypeVar_open]
+  | typeApp E' A =>
+    rw [TermVar_open, TypeVar_open, TermVar_open_TypeVar_open_eq, ← TermVar_open, ← TypeVar_open]
+
+theorem Term.TypeVar_open_Type'_open_eq {E : Term} {A : Type'}
+  (Alc : A.TypeVarLocallyClosed m) (mnen : m ≠ n)
+  : (E.TypeVar_open a m).Type'_open A n =
+    (E.Type'_open A n).TypeVar_open a m := by
+  match E with
+  | var _ => rw [TypeVar_open, Type'_open, TypeVar_open]
+  | lam A E' =>
+    rw [TypeVar_open, Type'_open, TypeVar_open_Type'_open_eq Alc mnen,
+        Type'.TypeVar_open_Type'_open_eq Alc mnen, ← TypeVar_open, ← Type'_open]
+  | app E' F =>
+    rw [TypeVar_open, Type'_open, TypeVar_open_Type'_open_eq Alc mnen,
+        TypeVar_open_Type'_open_eq Alc mnen, ← TypeVar_open, ← Type'_open]
+  | typeGen E' =>
+    rw [TypeVar_open, Type'_open]
+    simp only
+    rw [TypeVar_open_Type'_open_eq Alc.weaken (by exact mnen <| Nat.succ_inj'.mp ·), ← TypeVar_open,
+        ← Type'_open]
+  | typeApp E' A =>
+    rw [TypeVar_open, Type'_open, TypeVar_open_Type'_open_eq Alc mnen,
+        Type'.TypeVar_open_Type'_open_eq Alc mnen, ← TypeVar_open, ← Type'_open]
+
+inductive Term.TypeVarLocallyClosed : Term → Nat → Prop where
+  | var : TypeVarLocallyClosed (.var _) n
+  | lam : A.TypeVarLocallyClosed n → E.TypeVarLocallyClosed n → TypeVarLocallyClosed (lam A E) n
+  | app {E F : Term}
+    : E.TypeVarLocallyClosed n → F.TypeVarLocallyClosed n → TypeVarLocallyClosed (E.app F) n
+  | typeGen {E : Term} : E.TypeVarLocallyClosed (n + 1) → TypeVarLocallyClosed E.typeGen n
+  | typeApp {E : Term}
+    : E.TypeVarLocallyClosed n → A.TypeVarLocallyClosed n → TypeVarLocallyClosed (E.typeApp A) n
+
+theorem Term.TypeVarLocallyClosed.weaken {E : Term}
+  : E.TypeVarLocallyClosed m → E.TypeVarLocallyClosed (m + n)
+  | var => var
+  | lam Alc E'lc => lam Alc.weaken E'lc.weaken
+  | app E'lc Flc => app E'lc.weaken Flc.weaken
+  | typeGen E'lc => by
+    apply typeGen
+    rw [Nat.add_assoc, Nat.add_comm _ 1, ← Nat.add_assoc]
+    exact E'lc.weaken
+  | typeApp E'lc Alc => .typeApp E'lc.weaken Alc.weaken
+
+theorem Term.TypeVarLocallyClosed.TermVar_open_drop {E : Term}
+  : (E.TermVar_open x m).TypeVarLocallyClosed n → E.TypeVarLocallyClosed n := fun Elc => by
+  match E with
+  | .var _ => exact var
+  | .lam A' E' =>
+    rw [TermVar_open] at Elc
+    let .lam A'lc E'lc := Elc
+    exact lam A'lc E'lc.TermVar_open_drop
+  | .app E' F =>
+    rw [TermVar_open] at Elc
+    let .app E'lc Flc := Elc
+    exact app E'lc.TermVar_open_drop Flc.TermVar_open_drop
+  | .typeGen E' =>
+    rw [TermVar_open] at Elc
+    let .typeGen E'lc := Elc
+    exact typeGen E'lc.TermVar_open_drop
+  | .typeApp E' A =>
+    rw [TermVar_open] at Elc
+    let .typeApp E'lc A'lc := Elc
+    exact typeApp E'lc.TermVar_open_drop A'lc
+
+theorem Term.TypeVarLocallyClosed.TypeVar_open_drop {E : Term} (h : m < n)
+  : (E.TypeVar_open a m).TypeVarLocallyClosed n → E.TypeVarLocallyClosed n := fun Elc => by
+  match E with
+  | .var _ => exact var
+  | .lam A' E' =>
+    rw [TypeVar_open] at Elc
+    let .lam A'lc E'lc := Elc
+    exact lam (A'lc.TypeVar_open_drop h) (E'lc.TypeVar_open_drop h)
+  | .app E' F =>
+    rw [TypeVar_open] at Elc
+    let .app E'lc Flc := Elc
+    exact app (E'lc.TypeVar_open_drop h) (Flc.TypeVar_open_drop h)
+  | .typeGen E' =>
+    rw [TypeVar_open] at Elc
+    let .typeGen E'lc := Elc
+    exact typeGen <| E'lc.TypeVar_open_drop <| Nat.add_lt_add_iff_right.mpr h
+  | .typeApp E' A =>
+    rw [TypeVar_open] at Elc
+    let .typeApp E'lc A'lc := Elc
+    exact typeApp (E'lc.TypeVar_open_drop h) (A'lc.TypeVar_open_drop h)
+
+theorem Term.TypeVarLocallyClosed.TypeVar_open_eq {E : Term} (h : E.TypeVarLocallyClosed m)
+  (mlen : m ≤ n) : E.TypeVar_open x n = E := by match E, h with
+  | .var _, var => rw [TypeVar_open]
+  | .lam A E', lam Alc E'lc =>
+    rw [TypeVar_open, Alc.TypeVar_open_eq mlen, E'lc.TypeVar_open_eq mlen]
+  | .app E' F, app E'lc Flc =>
+    rw [TypeVar_open, E'lc.TypeVar_open_eq mlen, Flc.TypeVar_open_eq mlen]
+  | .typeGen E', typeGen E'lc =>
+    rw [TypeVar_open]
+    simp only
+    rw [E'lc.TypeVar_open_eq (Nat.add_le_add_iff_right.mpr mlen)]
+  | .typeApp E' A, typeApp E'lc Alc =>
+    rw [TypeVar_open, E'lc.TypeVar_open_eq mlen, Alc.TypeVar_open_eq mlen]
+
+theorem Term.TypeVar_open_TermVar_subst_eq {E F : Term} (Flc : F.TypeVarLocallyClosed n)
+  : (E.TypeVar_open x n).TermVar_subst x' F = (E.TermVar_subst x' F).TypeVar_open x n := by
+  match E with
+  | var x'' =>
+    rw [TypeVar_open, TermVar_subst]
+    split
+    · case isTrue h => exact Flc.TypeVar_open_eq (Nat.le_refl _) |>.symm
+    · case isFalse h => rw [TypeVar_open]
+  | lam A E' =>
+    rw [TypeVar_open, TermVar_subst, TermVar_subst, TypeVar_open,
+        E'.TypeVar_open_TermVar_subst_eq Flc]
+  | app E' F =>
+    rw [TypeVar_open, TermVar_subst, TermVar_subst, TypeVar_open,
+        E'.TypeVar_open_TermVar_subst_eq Flc, F.TypeVar_open_TermVar_subst_eq Flc]
+  | typeGen E' =>
+    rw [TypeVar_open, TermVar_subst, TermVar_subst, TypeVar_open,
+        E'.TypeVar_open_TermVar_subst_eq Flc.weaken]
+  | typeApp E' A =>
+    rw [TypeVar_open, TermVar_subst, TermVar_subst, TypeVar_open,
+        E'.TypeVar_open_TermVar_subst_eq Flc]
+
+theorem Term.TypeVar_open_Term_open_eq {E F : Term}
+  (Flc : F.TypeVarLocallyClosed n)
+  : (E.TypeVar_open x n).Term_open F m = (E.Term_open F m).TypeVar_open x n :=
+  by match E with
+  | var (.free _) => rw [TypeVar_open, Term_open, if_neg (nomatch ·), TypeVar_open]
+  | var (.bound _) =>
+    rw [TypeVar_open, Term_open]
+    split
+    · case isTrue h => rw [Flc.TypeVar_open_eq (Nat.le_refl _)]
+    · case isFalse h => rw [TypeVar_open]
+  | lam A E' =>
+    rw [TypeVar_open, Term_open]
+    simp only
+    rw [TypeVar_open_Term_open_eq Flc, Term_open, TypeVar_open]
+  | app E' F =>
+    rw [TypeVar_open, Term_open, TypeVar_open_Term_open_eq Flc, TypeVar_open_Term_open_eq Flc,
+        ← TypeVar_open, ← Term_open]
+  | typeGen E' =>
+    rw [TypeVar_open, Term_open, TypeVar_open_Term_open_eq Flc.weaken, ← TypeVar_open, Term_open]
+  | typeApp E' A =>
+    rw [TypeVar_open, Term_open, TypeVar_open_Term_open_eq Flc, ← TypeVar_open, Term_open]
+
 nosubst
 nonterminal Environment, G, D :=
   | "ε"                  : empty
-  | G ", " x " : " A     : termVarExt
-  | G ", " a             : typeVarExt
-  | G ", " D             : append (elab := return mkAppN (.const `LottExamples.SystemF.Environment.append []) #[G, D])
+  | G ", " x " : " A     : termVarExt (id x)
+  | G ", " a             : typeVarExt (id a)
+  | G ", " D             : append
+    (elab := return mkAppN (.const `LottExamples.SystemF.Environment.append []) #[G, D])
   | "(" G ")"            : paren (desugar := return G)
-  | G " [" A " / " a "]" : subst (elab := return mkAppN (.const `LottExamples.SystemF.Environment.subst []) #[G, a, A])
+  | G "^" a              : typeVarOpen (id a)
+    (elab := return mkAppN (.const `LottExamples.SystemF.Environment.TypeVar_open [])
+               #[G, a, .const `Nat.zero [] ])
+  | G "^^" A             : typeOpen
+    (elab := return mkAppN (.const `LottExamples.SystemF.Environment.Type'_open [])
+               #[G, A, .const `Nat.zero [] ])
 
-def Environment.append (G : Environment) : Environment → Environment
-  | .empty => G
-  | .termVarExt G' x A => G.append G' |>.termVarExt x A
-  | .typeVarExt G' a => G.append G' |>.typeVarExt a
+namespace Environment
 
-theorem Environment.empty_append (G : Environment) : G = Environment.empty.append G := by
-  induction G with
+def append (G : Environment) : Environment → Environment
+  | empty => G
+  | termVarExt G' x A => G.append G' |>.termVarExt x A
+  | typeVarExt G' a => G.append G' |>.typeVarExt a
+
+theorem append_termVarExt : [[(G, G', x : A)]] = [[((G, G'), x : A)]] := rfl
+
+theorem append_typeVarExt : [[(G, G', a)]] = [[((G, G'), a)]] := rfl
+
+theorem empty_append (G : Environment) : empty.append G = G :=
+  match G with
   | empty => rfl
-  | termVarExt G x A ih => congr
-  | typeVarExt G a ih => congr
+  | termVarExt G' x A => by rw [append_termVarExt, empty_append G']
+  | typeVarExt G' a => by rw [append_typeVarExt, empty_append G']
 
-def Environment.subst (G : Environment) (a : TypeVar) (A : Type') : Environment :=
-  go G |>.fst
-where
-  go
-    | Environment.empty => (Environment.empty, false)
-    | .termVarExt G' x A' =>
-      let (G'', found) := go G'
-      if found then
-        (G''.termVarExt x A', true)
-      else
-        (G''.termVarExt x (A'.TypeVar_subst a A), false)
-    | .typeVarExt G' a' =>
-      let (G'', found) := go G'
-      (G''.typeVarExt a', a' = a || found)
+theorem append_assoc : [[(G, G', G'')]] = [[((G, G'), G'')]] := match G'' with
+  | empty => rfl
+  | termVarExt G''' x A => by
+    rw [append_termVarExt, append_termVarExt, G.append_assoc, append_termVarExt]
+  | typeVarExt G''' a => by
+    rw [append_typeVarExt, append_typeVarExt, G.append_assoc, append_typeVarExt]
 
-theorem Environment.subst_empty : Environment.empty = Environment.empty.subst a A := rfl
+def Type'_open (G : Environment) (A : Type') (n : Nat) : Environment :=
+  match G, n with
+  | empty, _ => empty
+  | termVarExt G' x A', _ => G'.Type'_open A n |>.termVarExt x <| A'.Type'_open A n
+  | G@(typeVarExt ..), 0 => G
+  | typeVarExt G' a, n' + 1 => G'.Type'_open A n' |>.typeVarExt a
 
-theorem Environment.subst_typeVarExt_eq_typeVarExt_subst
-  : [[(G [B / b]), a]] = [[((G, a) [B / b])]] := rfl
+def TypeVar_open (G : Environment) (a : TypeVarId) (n : Nat) : Environment :=
+  match G, n with
+  | empty, _ => empty
+  | termVarExt G' x A', _ => G'.TypeVar_open a n |>.termVarExt x <| A'.TypeVar_open a n
+  | G@(typeVarExt ..), 0 => G
+  | typeVarExt G' a', n' + 1 => G'.TypeVar_open a n' |>.typeVarExt a'
+
+def termVar_count : Environment → Nat
+  | empty => 0
+  | termVarExt G _ _ => 1 + G.termVar_count
+  | typeVarExt G _ => G.termVar_count
+
+def typeVar_count : Environment → Nat
+  | empty => 0
+  | termVarExt G _ _ => G.typeVar_count
+  | typeVarExt G _ => 1 + G.typeVar_count
+
+end Environment
 
 nonterminal (parent := Term) Value, V :=
-  | "λ " x " : " A ". " E : lam
-  | "Λ " a ". " E         : typeGen
+  | "λ " x " : " A ". " E : lam (bind x in E)
+  | "Λ " a ". " E         : typeGen (bind a in E)
 
-judgement_syntax a " ≠ " b : TypeVarNe
+judgement_syntax a " ≠ " b : TypeVarNe (id a, b)
 
-def TypeVarNe := Ne (α := TypeVar)
+def TypeVarNe := Ne (α := TypeVarId)
 
-judgement_syntax a " ∈ " G : TypeVarInEnvironment
+judgement_syntax a " ∈ " G : TypeVarInEnvironment (id a)
 
 judgement TypeVarInEnvironment :=
 
@@ -108,11 +774,13 @@ a ≠ a'
 ───────── typeVarExt
 a ∈ G, a'
 
-judgement_syntax a " ∉ " G : TypeVarNotInEnvironment
+judgement_syntax a " ∉ " G : TypeVarNotInEnvironment (id a)
 
 def TypeVarNotInEnvironment a G := ¬[[a ∈ G]]
 
-theorem TypeVarInEnvironment.append_elim (ainGappGG : [[a ∈ G, GG]]) : [[a ∈ G]] ∨ [[a ∈ GG]] := by
+namespace TypeVarInEnvironment
+
+theorem append_elim (ainGappGG : [[a ∈ G, GG]]) : [[a ∈ G]] ∨ [[a ∈ GG]] := by
   by_cases [[a ∈ GG]]
   · case pos ainGG => exact .inr ainGG
   · case neg aninGG =>
@@ -131,7 +799,7 @@ theorem TypeVarInEnvironment.append_elim (ainGappGG : [[a ∈ G, GG]]) : [[a ∈
         apply False.elim
         apply aninGG
         rw [a'eqa]
-        exact .head
+        exact head
       · case neg a'nea =>
         apply ih
         · cases ainGappGG
@@ -142,7 +810,7 @@ theorem TypeVarInEnvironment.append_elim (ainGappGG : [[a ∈ G, GG]]) : [[a ∈
           have a'nea : a' ≠ a := a'nea
           exact ainGG'.typeVarExt a'nea.symm
 
-theorem TypeVarInEnvironment.append_inl (ainG : [[a ∈ G]]) : [[a ∈ G, GG]] := by
+theorem append_inl (ainG : [[a ∈ G]]) : [[a ∈ G, GG]] := by
   match GG with
   | .empty => exact ainG
   | .termVarExt GG' x A => exact ainG.append_inl |>.termVarExt
@@ -155,105 +823,46 @@ theorem TypeVarInEnvironment.append_inl (ainG : [[a ∈ G]]) : [[a ∈ G, GG]] :
       have a'nea : a' ≠ a := a'nea
       exact .typeVarExt ainG.append_inl a'nea.symm
 
-theorem TypeVarInEnvironment.append_inr : [[a ∈ GG]] → [[a ∈ G, GG]]
-  | .head => .head
-  | .termVarExt ainGG' => ainGG'.append_inr |>.termVarExt
-  | .typeVarExt ainGG' anea' => ainGG'.append_inr |>.typeVarExt anea'
+theorem append_inr : [[a ∈ GG]] → [[a ∈ G, GG]]
+  | head => head
+  | termVarExt ainGG' => ainGG'.append_inr |>.termVarExt
+  | typeVarExt ainGG' anea' => ainGG'.append_inr |>.typeVarExt anea'
 
-theorem TypeVarInEnvironment.subst (ainG : [[a ∈ G]]) : [[a ∈ G [A / b] ]] := by
-  rw [Environment.subst]
-  induction G
-  · case empty => cases ainG
-  · case termVarExt G' x A' ih =>
-    rw [Environment.subst.go]
-    simp
-    split <;>
-    · simp
-      apply TypeVarInEnvironment.termVarExt
-      apply ih
-      cases ainG
-      case a.termVarExt ainG' =>
-      exact ainG'
-  · case typeVarExt G' a' ih =>
-    rw [Environment.subst.go]
-    simp
-    cases ainG
-    · case head => exact .head
-    · case typeVarExt ainG' anea' =>
-      apply TypeVarInEnvironment.typeVarExt _ anea'
-      apply ih
-      exact ainG'
+theorem Type'_open {G : Environment}
+  : TypeVarInEnvironment a (G.TypeVar_open a' n) →
+    TypeVarInEnvironment a (G.Type'_open B n) := fun ainG => by
+  match G, n with
+  | .termVarExt .., _ =>
+    rw [Environment.Type'_open]
+    let .termVarExt ainG' := ainG
+    exact termVarExt ainG'.Type'_open
+  | .typeVarExt .., 0 =>
+    rw [Environment.Type'_open]
+    exact ainG
+  | .typeVarExt G' a', n' + 1 =>
+    rw [Environment.Type'_open]
+    match ainG with
+    | head => exact head
+    | typeVarExt ainG' anea' => exact typeVarExt ainG'.Type'_open anea'
 
-theorem TypeVarNotInEnvironment.termVarExt (aninG : [[a ∉ G]]) : [[a ∉ G, x : A]] := by
-  intro ainGx
-  apply aninG
-  cases ainGx
-  case termVarExt ainG => exact ainG
+end TypeVarInEnvironment
 
-theorem TypeVarNotInEnvironment.typeVarExt (aninG : [[a ∉ G]]) (bnea : b ≠ a) : [[a ∉ G, b]] := by
-  intro ainGa
-  apply aninG
-  cases ainGa
-  · case head => contradiction
-  · case typeVarExt ainG _ => exact ainG
+namespace TypeVarNotInEnvironment
 
-theorem TypeVarNotInEnvironment.TermVar_drop (aninGx : [[a ∉ G, x : A]]) : [[a ∉ G]] := by
-  intro ainG
-  exact aninGx ainG.termVarExt
+theorem termVarExt : [[a ∉ G]] → [[a ∉ G, x : A]]
+  | aninG, .termVarExt ainG => aninG ainG
 
-theorem TypeVarNotInEnvironment.TypeVar_drop (aninGb : [[a ∉ G, b]]) : [[a ∉ G]] := by
-  intro ainG
-  by_cases a = b
-  · case pos aeqb =>
-    rw [aeqb] at aninGb
-    exact aninGb .head
-  · case neg aneb => exact aninGb <| ainG.typeVarExt aneb
+theorem typeVarExt (h : a ≠ a') : [[a ∉ G]] → [[a ∉ G, a']]
+  | _, .head => h rfl
+  | aninG, .typeVarExt ainG _ => aninG ainG
 
-theorem Environment.subst_go_snd_eq_false_of_TermVarNotInEnvironment G (aninG : [[a ∉ G]])
-  : (Environment.subst.go a A G).snd = false := by
-  cases G
-  · case empty => rfl
-  · case termVarExt G' x A' =>
-    rw [subst.go]
-    split
-    split
-    · case isTrue q r found receq foundeqtrue =>
-      apply ne_false_of_eq_true (b := (subst.go a A G').snd)
-      · simp [foundeqtrue, receq]
-      · apply G'.subst_go_snd_eq_false_of_TermVarNotInEnvironment
-        exact aninG.TermVar_drop
-    · case isFalse => simp
-  · case typeVarExt G' a' =>
-    rw [subst.go]
-    simp
-    have a'nea : a' ≠ a := by
-      intro a'eqa
-      rw [a'eqa] at aninG
-      apply aninG
-      exact .head
-    constructor
-    · exact a'nea
-    · apply G'.subst_go_snd_eq_false_of_TermVarNotInEnvironment
-      exact aninG.TypeVar_drop
+end TypeVarNotInEnvironment
 
-theorem Environment.subst_termVarExt_eq_termVarExt_subst_of_TypeVarNotInEnvironment
-  (aninG : [[a ∉ G]]) : [[(G [B / a]), x : (A [B / a])]] = [[((G, x : A) [B / a])]] := by
-  rw [Environment.subst, Environment.subst, subst.go]
-  simp
-  split
-  · case isTrue sndeqtrue =>
-    apply False.elim
-    apply ne_false_of_eq_true sndeqtrue
-    exact G.subst_go_snd_eq_false_of_TermVarNotInEnvironment aninG
-  · case isFalse => simp
+judgement_syntax x " ≠ " y : TermVarNe (id x, y)
 
-theorem TypeVarNotInEnvironment.ε : [[a ∉ ε]] := fun ainε => by cases ainε
+def TermVarNe := Ne (α := TermVarId)
 
-judgement_syntax x " ≠ " y : TermVarNe
-
-def TermVarNe := Ne (α := TermVar)
-
-judgement_syntax x " : " A " ∈ " G : TermVarInEnvironment
+judgement_syntax x " : " A " ∈ " G : TermVarInEnvironment (id x)
 
 judgement TermVarInEnvironment :=
 
@@ -269,11 +878,13 @@ x : A ∈ G
 ──────────── typeVarExt
 x : A ∈ G, a
 
-judgement_syntax x " ∉ " G : TermVarNotInEnvironment
+judgement_syntax x " ∉ " G : TermVarNotInEnvironment (id x)
 
 def TermVarNotInEnvironment x G := ∀ A : Type', ¬[[x : A ∈ G]]
 
-theorem TermVarInEnvironment.append_elim (xAinGappGG : [[x : A ∈ G, GG]])
+namespace TermVarInEnvironment
+
+theorem append_elim (xAinGappGG : [[x : A ∈ G, GG]])
   : [[x : A ∈ G]] ∧ [[x ∉ GG]] ∨ [[x : A ∈ GG]] := by
   by_cases [[x : A ∈ GG]]
   · case pos xAinGG => exact .inr xAinGG
@@ -285,19 +896,19 @@ theorem TermVarInEnvironment.append_elim (xAinGappGG : [[x : A ∈ G, GG]])
       · exact xAinGappGG
       · intro A'
         intro xA'inε
-        cases xA'inε
+        nomatch xA'inε
     | .termVarExt GG' x' A' =>
       by_cases x' = x
       · case pos x'eqx =>
         by_cases A' = A
         · case pos A'eqA =>
           rw [x'eqx, A'eqA] at xAinGappGG xAninGG
-          exact False.elim <| xAninGG .head
+          exact xAninGG head |>.elim
         · case neg A'neA =>
           cases xAinGappGG
           · case head => contradiction
           · case termVarExt xAinGappGG' xnex' =>
-            exact False.elim <| xnex' x'eqx.symm
+            exact xnex' x'eqx.symm |>.elim
       · case neg x'nex =>
         cases xAinGappGG
         · case head => contradiction
@@ -308,8 +919,8 @@ theorem TermVarInEnvironment.append_elim (xAinGappGG : [[x : A ∈ G, GG]])
             · intro A''
               intro xA''inGG'x'A'
               match xA''inGG'x'A' with
-              | .head => contradiction
-              | .termVarExt xA''inG'  _ => exact xninGG' A'' xA''inG'
+              | head => contradiction
+              | termVarExt xA''inG'  _ => exact xninGG' A'' xA''inG'
           · have x'nex : x' ≠ x := x'nex
             exact False.elim <| xAninGG <| xAinG''.termVarExt x'nex.symm
     | .typeVarExt GG' a =>
@@ -325,9 +936,9 @@ theorem TermVarInEnvironment.append_elim (xAinGappGG : [[x : A ∈ G, GG]])
           case right.typeVarExt xA'inGG' =>
           exact xA'inGG'
       | .inr xAinGG' =>
-        exact False.elim <| xAninGG xAinGG'.typeVarExt
+        exact xAninGG xAinGG'.typeVarExt |>.elim
 
-theorem TermVarInEnvironment.append_inl (xAinG : [[x : A ∈ G]]) (xninGG : [[x ∉ GG]])
+theorem append_inl (xAinG : [[x : A ∈ G]]) (xninGG : [[x ∉ GG]])
   : [[x : A ∈ G, GG]] := by
   match GG with
   | .empty => exact xAinG
@@ -336,252 +947,50 @@ theorem TermVarInEnvironment.append_inl (xAinG : [[x : A ∈ G]]) (xninGG : [[x 
     · case pos x'eqx =>
       rw [x'eqx]
       rw [x'eqx] at xninGG
-      exact False.elim <| xninGG A' .head
+      exact False.elim <| xninGG A' head
     · case neg x'nex =>
       have x'nex : x' ≠ x := x'nex
       apply TermVarInEnvironment.termVarExt _ x'nex.symm
       apply xAinG.append_inl
       intro A'' xA''inGG'
       apply xninGG A''
-      exact .termVarExt xA''inGG' x'nex.symm
+      exact termVarExt xA''inGG' x'nex.symm
   | .typeVarExt GG' a =>
     apply TermVarInEnvironment.typeVarExt
     apply xAinG.append_inl
     intro A' xA'inGG'
     exact xninGG A' xA'inGG'.typeVarExt
 
-theorem TermVarInEnvironment.append_inr : [[x : A ∈ GG]] → [[x : A ∈ G, GG]]
-  | .head => .head
-  | .termVarExt xAinGG' xnex' => xAinGG'.append_inr |>.termVarExt xnex'
-  | .typeVarExt xAinGG' => xAinGG'.append_inr |>.typeVarExt
+theorem append_inr : [[x : A ∈ GG]] → [[x : A ∈ G, GG]]
+  | head => head
+  | termVarExt xAinGG' xnex' => xAinGG'.append_inr |>.termVarExt xnex'
+  | typeVarExt xAinGG' => xAinGG'.append_inr |>.typeVarExt
 
-theorem TermVarInEnvironment.TermVar_swap (x'inGxyGG : [[x' : A' ∈ G, x : A, y : B, GG]])
-  (xney : x ≠ y) : [[x' : A' ∈ G, y : B, x : A, GG]] := by
-  match x'inGxyGG.append_elim with
-  | .inl ⟨x'inGxy, x'ninGG⟩ =>
-    apply TermVarInEnvironment.append_inl _ x'ninGG
-    match x'inGxy with
-    | .head => exact .termVarExt .head xney.symm
-    | .termVarExt x'inGx x'ney => match x'inGx with
-      | .head => exact .head
-      | .termVarExt x'inG x'nex => exact x'inG.termVarExt x'ney |>.termVarExt x'nex
-  | .inr x'inGG => exact x'inGG.append_inr
+theorem Type'_open {A : Type'} {G : Environment}
+  : TermVarInEnvironment x (A.TypeVar_open a n) (G.TypeVar_open a n) →
+    TermVarInEnvironment x (A.Type'_open B n) (G.Type'_open B n) := sorry
 
-theorem TermVarInEnvironment.subst (xAinG : [[x : A ∈ G]]) (aninG : [[a ∉ G]])
-  : [[x : A [B / a] ∈ G [B / a] ]] := by
-  rw [Environment.subst]
-  induction G
-  · case empty => cases xAinG
-  · case termVarExt G' x' A' ih =>
-    rw [Environment.subst.go]
-    simp
-    split
-    · case isTrue sndeqtrue =>
-      apply False.elim
-      apply ne_false_of_eq_true sndeqtrue
-      apply G'.subst_go_snd_eq_false_of_TermVarNotInEnvironment
-      exact aninG.TermVar_drop
-    · case isFalse sndeqfalse =>
-      cases xAinG
-      · case head => exact .head
-      · case termVarExt xAinG' xnex' =>
-        apply TermVarInEnvironment.termVarExt _ xnex'
-        apply ih xAinG'
-        exact aninG.TermVar_drop
-  · case typeVarExt G' a' ih =>
-    rw [Environment.subst.go]
-    simp
-    cases xAinG
-    case typeVarExt xAinG' =>
-    apply TermVarInEnvironment.typeVarExt
-    apply ih xAinG'
-    exact aninG.TypeVar_drop
+end TermVarInEnvironment
 
-theorem TermVarInEnvironment.unsubst (xAsinGs : [[x : A' ∈ G [B / a] ]]) (aninG : [[a ∉ G]])
-  : ∃ A, [[x : A ∈ G]] ∧ A' = [[(A [B / a])]] := by
-  rw [Environment.subst] at xAsinGs
-  induction G
-  · case empty => cases xAsinGs
-  · case termVarExt G' x' A' ih =>
-    rw [Environment.subst.go] at xAsinGs
-    simp at xAsinGs
-    split at xAsinGs
-    · case isTrue sndeqtrue =>
-      apply False.elim
-      apply ne_false_of_eq_true sndeqtrue
-      apply G'.subst_go_snd_eq_false_of_TermVarNotInEnvironment
-      exact aninG.TermVar_drop
-    · case isFalse sndeqfalse =>
-      simp at xAsinGs
-      cases xAsinGs
-      · case head => exact Exists.intro A' ⟨.head, rfl⟩
-      · case termVarExt xAinG' xnex' =>
-        let ⟨A'', ⟨xA''inG', eq⟩⟩ := ih xAinG' aninG.TermVar_drop
-        exact Exists.intro A'' ⟨xA''inG'.termVarExt xnex', eq⟩
-  · case typeVarExt G' a' ih =>
-    rw [Environment.subst.go] at xAsinGs
-    simp at xAsinGs
-    cases xAsinGs
-    case typeVarExt xAinG' =>
-    let ⟨A', ⟨xA'inG', eq⟩⟩ := ih xAinG' aninG.TypeVar_drop
-    exact Exists.intro A' ⟨xA'inG'.typeVarExt, eq⟩
+namespace TermVarNotInEnvironment
 
-theorem TermVarNotInEnvironment.ε : [[x ∉ ε]] := fun _ xinε => by cases xinε
-
-theorem TermVarNotInEnvironment.termVarExt (xninG : [[x ∉ G]]) (ynex : y ≠ x)
-  : [[x ∉ G, y : A]] := by
-  intro A' xA'inGy
-  apply xninG A'
-  cases xA'inGy
+theorem termVarExt (xnex' : x ≠ x') : [[x ∉ G]] → [[x ∉ G, x' : A]] := fun xnin A xAinGx'A => by
+  apply xnin A
+  cases xAinGx'A
   · case head => contradiction
-  · case termVarExt xA'inG _ => exact xA'inG
+  · case termVarExt h _ => exact h
 
-theorem TermVarNotInEnvironment.typeVarExt (xninG : [[x ∉ G]]) : [[x ∉ G, a]] := by
-  intro A' xA'inGa
-  apply xninG A'
-  cases xA'inGa
-  case typeVarExt xA'inG => exact xA'inG
+theorem typeVarExt : [[x ∉ G]] → [[x ∉ G, a]] := fun xnin A xAinGa => by
+  apply xnin A
+  cases xAinGa
+  case typeVarExt h =>
+  exact h
 
-judgement_syntax G " ⊢ " A : TypeWellFormedness
+end TermVarNotInEnvironment
 
-judgement TypeWellFormedness :=
+judgement_syntax a " ∈ " "ftv" "(" A ")" : InTypeFreeTypeVars (id a)
 
-a ∈ G
-───── var
-G ⊢ a
-
-G ⊢ A
-G ⊢ B
-───────── arr
-G ⊢ A → B
-
-G, a ⊢ A
-────────── forall'
-G ⊢ ∀ a. A
-
-theorem TypeWellFormedness.TypeVar_swap (Awf : [[G, b, a, GG ⊢ A]]) : [[G, a, b, GG ⊢ A]] := by
-  cases Awf
-  · case var a' a'inGbaGG =>
-    match a'inGbaGG.append_elim with
-    | .inl a'inGba =>
-      cases a'inGba
-      · case head =>
-        by_cases a = b
-        · case pos aeqb =>
-          rw [aeqb]
-          exact .var TypeVarInEnvironment.head.append_inl
-        · case neg aneb =>
-          exact .var <| .append_inl <| .typeVarExt .head aneb
-      · case typeVarExt a'inGb a'nea =>
-        cases a'inGb
-        · case head => exact .var <| .append_inl .head
-        · case typeVarExt a'inG a'neb =>
-          exact .var <| .append_inl <| .typeVarExt (.typeVarExt a'inG a'nea) a'neb
-    | .inr a'inGG => exact .var a'inGG.append_inr
-  · case arr A' B A'wf Bwf =>
-    exact .arr A'wf.TypeVar_swap Bwf.TypeVar_swap
-  · case forall' a' A' A'wf =>
-    apply TypeWellFormedness.forall'
-    rw [← Environment.append]
-    exact TypeWellFormedness.TypeVar_swap A'wf
-
-theorem TypeWellFormedness.TypeVar_shadowed : [[G, a, a ⊢ A]] → [[G, a ⊢ A]]
-  | .var a'inGaa => match a'inGaa with
-    | .head => .var .head
-    | .typeVarExt a'inGa _ => .var a'inGa
-  | .arr A'wf Bwf => .arr A'wf.TypeVar_shadowed Bwf.TypeVar_shadowed
-  | .forall' A'wf => .forall' <| A'wf.TypeVar_swap (GG := .empty)
-      |>.TypeVar_swap (GG := .typeVarExt .empty a)
-      |>.TypeVar_shadowed
-      |>.TypeVar_swap (GG := .empty)
-
-theorem TypeWellFormedness.TermVar_drop : [[G, x : A, GG ⊢ B]] → [[G, GG ⊢ B]]
-  | .var ainGxGG => match ainGxGG.append_elim with
-    | .inl (.termVarExt ainG) => .var ainG.append_inl
-    | .inr ainGG => .var ainGG.append_inr
-  | .arr A'wf B'wf => .arr A'wf.TermVar_drop B'wf.TermVar_drop
-  | .forall' A'wf => .forall' <| A'wf.TermVar_drop (GG := .typeVarExt GG _)
-
-theorem TypeWellFormedness.TermVar_intro : [[G, GG ⊢ B]] → [[G, x : A, GG ⊢ B]]
-  | .var ainGappGG => match ainGappGG.append_elim with
-    | .inl ainG => .var ainG.termVarExt.append_inl
-    | .inr ainGG => .var ainGG.append_inr
-  | .arr A'wf B'wf => .arr A'wf.TermVar_intro B'wf.TermVar_intro
-  | .forall' A'wf => .forall' <| A'wf.TermVar_intro (GG := .typeVarExt GG _)
-
-theorem TypeWellFormedness.TermVar_swap (Bwf : [[G, y : A', x : A, GG ⊢ B]])
-  : [[G, x : A, y : A', GG ⊢ B]] := Bwf.TermVar_drop.TermVar_drop.TermVar_intro.TermVar_intro
-
-theorem TypeWellFormedness.append_inr : [[G ⊢ A]] → [[GG, G ⊢ A]]
-  | .var ainG => .var ainG.append_inr
-  | .arr A'wf Bwf => .arr A'wf.append_inr Bwf.append_inr
-  | .forall' A'wf => .forall' A'wf.append_inr
-
-theorem TypeWellFormedness.TypeVar_shadowed_subst
-  : [[ε, a, G, a, GG ⊢ A]] → [[(G, a) [B / a], GG ⊢ A]]
-  | .var a'inεaGaGG =>
-    match a'inεaGaGG.append_elim with
-    | .inl a'inεa =>
-      match a'inεa with
-      | .head => .var TypeVarInEnvironment.head.subst.append_inl
-      | .typeVarExt a'inε _ => by cases a'inε
-    | .inr a'inGaGG => match a'inGaGG.append_elim with
-      | .inl a'inGa => .var a'inGa.subst.append_inl
-      | .inr a'inGG => .var a'inGG.append_inr
-  | .arr A'wf B'wf => .arr A'wf.TypeVar_shadowed_subst B'wf.TypeVar_shadowed_subst
-  | .forall' A'wf => .forall' <| A'wf.TypeVar_shadowed_subst (GG := GG.typeVarExt _)
-
-theorem TypeWellFormedness.subst (Awf : [[ε, a, G ⊢ A]]) (Bwf : [[ε ⊢ B]])
-  : [[G [B / a] ⊢ A [B / a] ]] := by
-  cases Awf
-  · case var a' a'inεaG =>
-    rw [Type'.TypeVar_subst]
-    split
-    · case isTrue a'eqa =>
-      exact Bwf.append_inr
-    · case isFalse a'nea =>
-      match a'inεaG.append_elim with
-      | .inl a'inεa =>
-        cases a'inεa
-        · case head => contradiction
-        · case typeVarExt => contradiction
-      | .inr a'inG =>
-        exact .var a'inG.subst
-  · case arr A' B' A'wf B'wf => exact .arr (A'wf.subst Bwf) (B'wf.subst Bwf)
-  · case forall' a' A' A'wf =>
-    rw [Type'.TypeVar_subst]
-    split
-    · case isTrue a'eqa =>
-      rw [a'eqa]
-      rw [a'eqa] at A'wf
-      exact .forall' <| A'wf.TypeVar_shadowed_subst (GG := .empty)
-    · case isFalse a'nea => exact TypeWellFormedness.forall' <| A'wf.subst (G := G.typeVarExt a') Bwf
-
-theorem Type'.subst_id_of_TypeWellFormedness_of_TypeVarNotInEnvironment (Awf : [[G ⊢ A]])
-  (aninG : [[a ∉ G]]) : [[(A [B / a])]] = A := by
-  match Awf with
-  | .var a'inG =>
-    rw [Type'.TypeVar_subst]
-    split
-    · case isTrue aeqa' =>
-      rw [aeqa'.symm] at a'inG
-      exact False.elim <| aninG a'inG
-    · case isFalse => rfl
-  | .arr A'wf B'wf =>
-    rw [Type'.TypeVar_subst, Type'.subst_id_of_TypeWellFormedness_of_TypeVarNotInEnvironment A'wf aninG,
-        Type'.subst_id_of_TypeWellFormedness_of_TypeVarNotInEnvironment B'wf aninG]
-  | .forall' A'wf =>
-    rw [Type'.TypeVar_subst]
-    split
-    · case isTrue => rfl
-    · case isFalse anea' =>
-      rw [Type'.subst_id_of_TypeWellFormedness_of_TypeVarNotInEnvironment A'wf]
-      have anea' : a ≠ _ := anea'
-      exact aninG.typeVarExt anea'.symm
-
-judgement_syntax a " ∈ " "ftv" "(" A ")" : InFreeTypeVars
-
-judgement InFreeTypeVars :=
+judgement InTypeFreeTypeVars :=
 
 ────────── var
 a ∈ ftv(a)
@@ -595,80 +1004,123 @@ a ∈ ftv(B)
 a ∈ ftv(A → B)
 
 a ∈ ftv(A)
-a ≠ b
 ─────────────── forall'
 a ∈ ftv(∀ b. A)
 
-judgement_syntax a " ∉ " "ftv" "(" A ")" : NotInFreeTypeVars
+namespace InTypeFreeTypeVars
 
-def NotInFreeTypeVars a A := ¬[[a ∈ ftv(A)]]
-
-theorem NotInFreeTypeVars.of_TypeWellFormedness_of_TypeVarNotInEnvironment (Awf : [[G ⊢ A]])
-  (aninG : [[a ∉ G]]) : [[a ∉ ftv(A)]] := by
-  intro ain
-  match A, Awf with
-  | .var a', .var a'inG =>
-    let .var := ain
-    exact aninG a'inG
-  | .arr A' B, .arr A'wf Bwf => match ain with
-    | .arrl ainA' =>
-      exact NotInFreeTypeVars.of_TypeWellFormedness_of_TypeVarNotInEnvironment A'wf aninG <| ainA'
-    | .arrr ainB =>
-      exact NotInFreeTypeVars.of_TypeWellFormedness_of_TypeVarNotInEnvironment Bwf aninG <| ainB
-  | .forall' a' A', .forall' A'wf =>
-    let .forall' ainftvA' anea' := ain
-    apply NotInFreeTypeVars.of_TypeWellFormedness_of_TypeVarNotInEnvironment A'wf _ ainftvA'
-    exact aninG.typeVarExt anea'.symm
-
-theorem InFreeTypeVars.unsubst (ain : [[a ∈ ftv(A [B / b])]]) (Bwf : [[ε ⊢ B]]) : [[a ∈ ftv(A)]] := by
+theorem of_TypeVar_open {A : Type'} (h : a ≠ a')
+  : InTypeFreeTypeVars a (A.TypeVar_open a' n) → [[a ∈ ftv(A)]] := fun ainAop => by
   match A with
-  | .var a' =>
-    rw [Type'.TypeVar_subst] at ain
-    split at ain
-    · case isTrue a'eqa =>
-      exact False.elim <|
-        NotInFreeTypeVars.of_TypeWellFormedness_of_TypeVarNotInEnvironment Bwf
-          TypeVarNotInEnvironment.ε ain
-    · case isFalse a'neb =>
-      let .var := ain
-      exact .var
-  | .arr A' B' =>
-    rw [Type'.TypeVar_subst] at ain
-    match ain with
-    | .arrl ain => exact .arrl <| ain.unsubst Bwf
-    | .arrr ain => exact .arrr <| ain.unsubst Bwf
-  | .forall' a' A' =>
-    rw [Type'.TypeVar_subst] at ain
-    split at ain
-    · case isTrue a'eqb => exact ain
-    · case isFalse a'neb =>
-      let .forall' ain anea' := ain
-      exact .forall' (ain.unsubst Bwf) anea'
+  | .var (.free _) =>
+    rw [Type'.TypeVar_open] at ainAop
+    let .var := ainAop
+    exact .var
+  | .var (.bound _) =>
+    rw [Type'.TypeVar_open] at ainAop
+    split at ainAop
+    · case isTrue h =>
+      cases ainAop
+      contradiction
+    · case isFalse h =>
+      nomatch ainAop
+  | .arr A' B =>
+    rw [Type'.TypeVar_open] at ainAop
+    match ainAop with
+    | .arrl ainA'op => exact .arrl <| ainA'op.of_TypeVar_open h
+    | .arrr ainA'op => exact .arrr <| ainA'op.of_TypeVar_open h
+  | .forall' A' =>
+    rw [Type'.TypeVar_open] at ainAop
+    let .forall' ainA'op := ainAop
+    exact .forall' <| ainA'op.of_TypeVar_open h
 
-theorem NotInFreeTypeVars.subst_id (aninftvA : [[a ∉ ftv(A)]]) : [[(A [B / a])]] = A := by
+theorem exists_gt (A : Type') : ∃ a : Nat, ∀ a' : Nat, [[a' ∈ ftv(A)]] → a' < a :=
   match A with
-  | .var a' =>
-    rw [Type'.TypeVar_subst, if_neg]
-    intro a'eqa
-    rw [a'eqa] at aninftvA
-    exact aninftvA .var
-  | .arr A' B' =>
-    rw [Type'.TypeVar_subst, NotInFreeTypeVars.subst_id, NotInFreeTypeVars.subst_id]
-    · intro ainftvB'
-      exact aninftvA <| .arrr ainftvB'
-    · intro ainftvA'
-      exact aninftvA <| .arrl ainftvA'
-  | .forall' a' A' =>
-    rw [Type'.TypeVar_subst]
-    split
-    · case isTrue => rfl
-    · case isFalse a'nea =>
-      have a'nea : a ≠ a' := a'nea
-      rw [NotInFreeTypeVars.subst_id]
-      intro ainftvA'
-      exact aninftvA <| InFreeTypeVars.forall' ainftvA' a'nea
+  | .var (.free (x : Nat)) =>
+    .intro (x + 1) fun | x', .var => Nat.lt_succ_self _
+  | .var (.bound _) => .intro 0 fun _ x'in => nomatch x'in
+  | .arr E' F =>
+    let ⟨xE', xE'gt⟩ := exists_gt E'
+    let ⟨xF, xFgt⟩ := exists_gt F
+    .intro (max xE' xF) fun
+      | x', .arrl x'infvE' =>
+        Nat.lt_of_lt_of_le (xE'gt x' x'infvE') <| Nat.le_max_left _ _
+      | x', .arrr x'infvF =>
+        Nat.lt_of_lt_of_le (xFgt x' x'infvF) <| Nat.le_max_right _ _
+  | .forall' E' =>
+    let ⟨xE', xE'gt⟩ := exists_gt E'
+    .intro xE' fun | _, .forall' x'infvE' => xE'gt _ x'infvE'
 
-judgement_syntax x " ∈ " "fv" "(" E ")" : InFreeTermVars
+end InTypeFreeTypeVars
+
+judgement_syntax a " ∉ " "ftv" "(" A ")" : NotInTypeFreeTypeVars (id a)
+
+def NotInTypeFreeTypeVars a A := ¬[[a ∈ ftv(A)]]
+
+namespace NotInTypeFreeTypeVars
+
+theorem arr : [[a ∉ ftv(A → B)]] ↔ [[a ∉ ftv(A)]] ∧ [[a ∉ ftv(B)]] := ⟨
+    fun anin => ⟨(anin <| .arrl ·), (anin <| .arrr ·)⟩,
+    fun
+      | ⟨aninA, _⟩, .arrl ainA => aninA ainA
+      | ⟨_, aninB⟩, .arrr ainB => aninB ainB
+  ⟩
+
+theorem forall' : [[a ∉ ftv(∀ b. A)]] → [[a ∉ ftv(A)]] := (· <| .forall' ·)
+
+theorem TypeVar_open_of_ne (h : a ≠ a') : [[a ∉ ftv(A)]] → [[a ∉ ftv(A^a')]] :=
+  (· <| ·.of_TypeVar_open h)
+
+theorem TypeVar_open_inj_of {A B : Type'} (aninftvA : [[a ∉ ftv(A)]]) (aninftvB : [[a ∉ ftv(B)]])
+  : A.TypeVar_open a n = B.TypeVar_open a n → A = B := by
+  intro AopeqBop
+  match A, B with
+  | .var (.free _), .var (.free _) =>
+    rw [Type'.TypeVar_open, if_neg (nomatch ·), Type'.TypeVar_open, if_neg (nomatch ·)] at AopeqBop
+    exact AopeqBop
+  | .var (.free _), .var (.bound _) =>
+    rw [Type'.TypeVar_open, if_neg (nomatch ·), Type'.TypeVar_open] at AopeqBop
+    split at AopeqBop
+    · case isTrue h =>
+      rw [Type'.var.inj AopeqBop] at aninftvA
+      exact aninftvA .var |>.elim
+    · case isFalse h => nomatch AopeqBop
+  | .var (.bound _), .var (.free _) =>
+    rw [Type'.TypeVar_open] at AopeqBop
+    split at AopeqBop
+    · case isTrue h =>
+      rw [Type'.TypeVar_open, if_neg (nomatch ·)] at AopeqBop
+      rw [← Type'.var.inj AopeqBop] at aninftvB
+      exact aninftvB .var |>.elim
+    · case isFalse h => nomatch AopeqBop
+  | .var (.bound _), .var (.bound _) =>
+    rw [Type'.TypeVar_open] at AopeqBop
+    split at AopeqBop
+    · case isTrue h =>
+      rw [← h]
+      rw [Type'.TypeVar_open] at AopeqBop
+      split at AopeqBop
+      · case isTrue h' => rw [← h']
+      · case isFalse h' => nomatch AopeqBop
+    · case isFalse h =>
+      rw [Type'.TypeVar_open] at AopeqBop
+      split at AopeqBop
+      · case isTrue h' => nomatch AopeqBop
+      · case isFalse h' => exact AopeqBop
+  | .arr A' B', .arr A'' B'' =>
+    rw [Type'.TypeVar_open, Type'.TypeVar_open] at AopeqBop
+    let ⟨A'opeqA''op, B'opeqB''op⟩ := Type'.arr.inj AopeqBop
+    rw [(NotInTypeFreeTypeVars.arr.mp aninftvA).left.TypeVar_open_inj_of
+          (NotInTypeFreeTypeVars.arr.mp aninftvB).left A'opeqA''op,
+        (NotInTypeFreeTypeVars.arr.mp aninftvA).right.TypeVar_open_inj_of
+          (NotInTypeFreeTypeVars.arr.mp aninftvB).right B'opeqB''op]
+  | .forall' A', .forall' A'' =>
+    rw [Type'.TypeVar_open, Type'.TypeVar_open] at AopeqBop
+    rw [aninftvA.forall'.TypeVar_open_inj_of aninftvB.forall' <| Type'.forall'.inj AopeqBop]
+
+end NotInTypeFreeTypeVars
+
+judgement_syntax x " ∈ " "fv" "(" E ")" : InFreeTermVars (id x)
 
 judgement InFreeTermVars :=
 
@@ -676,7 +1128,6 @@ judgement InFreeTermVars :=
 x ∈ fv(x)
 
 x ∈ fv(E)
-x ≠ y
 ────────────────── lam
 x ∈ fv(λ y : A. E)
 
@@ -696,97 +1147,360 @@ x ∈ fv(E)
 ───────────── typeApp
 x ∈ fv(E [A])
 
-judgement_syntax x " ∉ " "fv" "(" E ")" : NotInFreeTermVars
+namespace InFreeTermVars
+
+theorem of_TermVar_open {E : Term} (h : x ≠ x')
+  : InFreeTermVars x (E.TermVar_open x' n) → [[x ∈ fv(E)]] := fun xinEop => by
+  match E with
+  | .var (.free _) =>
+    rw [Term.TermVar_open] at xinEop
+    let .var := xinEop
+    exact .var
+  | .var (.bound _) =>
+    rw [Term.TermVar_open] at xinEop
+    split at xinEop
+    · case isTrue h =>
+      cases xinEop
+      contradiction
+    · case isFalse h =>
+      nomatch xinEop
+  | .lam A E' =>
+    rw [Term.TermVar_open] at xinEop
+    let .lam xinE'op := xinEop
+    exact .lam <| xinE'op.of_TermVar_open h
+  | .app E' F =>
+    rw [Term.TermVar_open] at xinEop
+    match xinEop with
+    | .appl xinE'op => exact .appl <| xinE'op.of_TermVar_open h
+    | .appr xinE'op => exact .appr <| xinE'op.of_TermVar_open h
+  | .typeGen E' =>
+    rw [Term.TermVar_open] at xinEop
+    let .typeGen xinE'op := xinEop
+    exact .typeGen <| xinE'op.of_TermVar_open h
+  | .typeApp E' A =>
+    rw [Term.TermVar_open] at xinEop
+    let .typeApp xinE'op := xinEop
+    exact .typeApp <| xinE'op.of_TermVar_open h
+
+theorem of_TypeVar_open {E : Term}
+  : InFreeTermVars x (E.TypeVar_open a n) → [[x ∈ fv(E)]] := fun xinEop => by
+  match E with
+  | .var _ =>
+    rw [Term.TypeVar_open] at xinEop
+    let .var := xinEop
+    exact .var
+  | .lam A E' =>
+    rw [Term.TypeVar_open] at xinEop
+    let .lam xinE'op := xinEop
+    exact .lam xinE'op.of_TypeVar_open
+  | .app E' F =>
+    rw [Term.TypeVar_open] at xinEop
+    match xinEop with
+    | .appl xinE'op => exact .appl xinE'op.of_TypeVar_open
+    | .appr xinE'op => exact .appr xinE'op.of_TypeVar_open
+  | .typeGen E' =>
+    rw [Term.TypeVar_open] at xinEop
+    let .typeGen xinE'op := xinEop
+    exact .typeGen xinE'op.of_TypeVar_open
+  | .typeApp E' A =>
+    rw [Term.TypeVar_open] at xinEop
+    let .typeApp xinE'op := xinEop
+    exact .typeApp xinE'op.of_TypeVar_open
+
+theorem exists_gt (E : Term) : ∃ x : Nat, ∀ x' : Nat, [[x' ∈ fv(E)]] → x' < x :=
+  match E with
+  | .var (.free (x : Nat)) =>
+    .intro (x + 1) fun | x', .var => Nat.lt_succ_self _
+  | .var (.bound _) => .intro 0 fun _ x'in => nomatch x'in
+  | .lam _ E' =>
+    let ⟨xE', xE'gt⟩ := exists_gt E'
+    .intro xE' fun | _, .lam x'infvE' => xE'gt _ x'infvE'
+  | .app E' F =>
+    let ⟨xE', xE'gt⟩ := exists_gt E'
+    let ⟨xF, xFgt⟩ := exists_gt F
+    .intro (max xE' xF) fun
+      | x', .appl x'infvE' =>
+        Nat.lt_of_lt_of_le (xE'gt x' x'infvE') <| Nat.le_max_left _ _
+      | x', .appr x'infvF =>
+        Nat.lt_of_lt_of_le (xFgt x' x'infvF) <| Nat.le_max_right _ _
+  | .typeGen E' =>
+    let ⟨xE', xE'gt⟩ := exists_gt E'
+    .intro xE' fun | _, .typeGen x'infvE' => xE'gt _ x'infvE'
+  | .typeApp E' _ =>
+    let ⟨xE', xE'gt⟩ := exists_gt E'
+    .intro xE' fun | _, .typeApp x'infvE' => xE'gt _ x'infvE'
+
+end InFreeTermVars
+
+judgement_syntax x " ∉ " "fv" "(" E ")" : NotInFreeTermVars (id x)
 
 def NotInFreeTermVars x E := ¬[[x ∈ fv(E)]]
 
-judgement_syntax G " ⊢ " a " ∈ " "fvftv" "(" E ")" : InFreeTermVars'Types'FreeTypeVars
+namespace NotInFreeTermVars
 
-judgement InFreeTermVars'Types'FreeTypeVars :=
+theorem lam : [[x ∉ fv(λ y : A. E)]] → [[x ∉ fv(E)]] := (· <| .lam ·)
 
-x ∈ fv(E)
-x : A ∈ G
+theorem app : [[x ∉ fv(E F)]] → ([[x ∉ fv(E)]] ∧ [[x ∉ fv(F)]]) :=
+  fun xnin => ⟨(xnin <| .appl ·), (xnin <| .appr ·)⟩
+
+theorem typeGen : [[x ∉ fv(Λ a. E)]] → [[x ∉ fv(E)]] := (· <| .typeGen ·)
+
+theorem typeApp : [[x ∉ fv(E [A])]] → [[x ∉ fv(E)]] := (· <| .typeApp ·)
+
+theorem TermVar_open_of_ne (h : x ≠ x') : [[x ∉ fv(E)]] → [[x ∉ fv(E^x')]] :=
+  (· <| ·.of_TermVar_open h)
+
+theorem TypeVar_open : [[x ∉ fv(E)]] → [[x ∉ fv(E^a)]] := (· ·.of_TypeVar_open)
+
+theorem exists_fresh {I : List _} : ∃ x ∉ I, [[x ∉ fv(E)]] :=
+  let ⟨xI, xIgt⟩ := I.exists_gt
+  let ⟨xE, xEgt⟩ := InFreeTermVars.exists_gt E
+  let xIE := max xI xE
+  .intro xIE ⟨
+    fun inI => Nat.not_le_of_lt (xIgt xIE inI) <| Nat.le_max_left _ _,
+    fun inE => Nat.not_le_of_lt (xEgt xIE inE) <| Nat.le_max_right _ _
+  ⟩
+
+end NotInFreeTermVars
+
+judgement_syntax a " ∈ " "ftv" "(" E ")" : InTermFreeTypeVars (id a)
+
+judgement InTermFreeTypeVars :=
+
 a ∈ ftv(A)
-──────────────── mk
-G ⊢ a ∈ fvftv(E)
+─────────────────── laml
+a ∈ ftv(λ x : A. E)
 
-judgement_syntax G " ⊢ " a " ∉ " "fvftv" "(" E ")" : NotInFreeTermVars'Types'FreeTypeVars
+a ∈ ftv(E)
+─────────────────── lamr
+a ∈ ftv(λ x : A. E)
 
-def NotInFreeTermVars'Types'FreeTypeVars G a E := ¬[[G ⊢ a ∈ fvftv(E)]]
+a ∈ ftv(E)
+──────────── appl
+a ∈ ftv(E F)
 
-theorem NotInFreeTermVars'Types'FreeTypeVars.TermVar_swap
-  (anin : [[G, y : A', x : A, GG ⊢ a ∉ fvftv(E)]]) (xney : x ≠ y)
-  : [[G, x : A, y : A', GG ⊢ a ∉ fvftv(E)]] := by
-  intro ain
-  apply anin
-  let .mk x'infv x'A'in ainftvA' := ain
-  exact InFreeTermVars'Types'FreeTypeVars.mk x'infv (x'A'in.TermVar_swap xney) ainftvA'
+a ∈ ftv(F)
+──────────── appr
+a ∈ ftv(E F)
 
-theorem NotInFreeTermVars'Types'FreeTypeVars.TermVar_shadowed (anin : [[G, x : A_shadowed, GG, x : A, GGG ⊢ a ∉ fvftv(E)]])
-  : [[G, GG, x : A, GGG ⊢ a ∉ fvftv(E)]] := by
-  intro ain
-  apply anin
-  cases ain
-  case mk x' A' x'A'in ainftvA' x'infv =>
-  apply InFreeTermVars'Types'FreeTypeVars.mk x'infv _ ainftvA'
-  match x'A'in.append_elim with
-  | .inl ⟨x'A'inG, x'ninGGxGGG⟩ =>
-    apply TermVarInEnvironment.append_inl _ x'ninGGxGGG
-    by_cases x' = x
-    · case pos x'eqx =>
-      apply False.elim
-      rw [x'eqx] at x'ninGGxGGG
-      apply x'ninGGxGGG A
-      apply TermVarInEnvironment.head.append_inl
-      intro A'' xA''inGG
-      apply x'ninGGxGGG A''
-      exact xA''inGG.append_inr
-    · case neg x'nex => exact x'A'inG.termVarExt x'nex
-  | .inr x'A'inGGxGGG => exact x'A'inGGxGGG.append_inr
+a ∈ ftv(E)
+─────────────── typeGen
+a ∈ ftv(Λ a. E)
 
-theorem NotInFreeTermVars'Types'FreeTypeVars.append_elr (anin : [[G, GG ⊢ a ∉ fvftv(E)]])
-  : [[GG ⊢ a ∉ fvftv(E)]] := by
-  intro ain
-  apply anin
-  let .mk x'infv x'A'inG ainftv := ain
-  exact InFreeTermVars'Types'FreeTypeVars.mk x'infv x'A'inG.append_inr ainftv
+a ∈ ftv(E)
+────────────── typeAppl
+a ∈ ftv(E [A])
 
-theorem NotInFreeTermVars'Types'FreeTypeVars.Environment_subst (anin : [[G ⊢ a ∉ fvftv(E)]])
-  (Awf : [[ε ⊢ A]]) (bninG : [[b ∉ G]]) : [[G [A / b] ⊢ a ∉ fvftv(E)]] := by
-  intro ain
-  apply anin
-  let .mk x'infv x'A'inG ainftv := ain
-  let ⟨_, ⟨xA'inG', eq⟩⟩ := x'A'inG.unsubst bninG
-  rw [eq] at ainftv
-  exact .mk x'infv xA'inG' <| ainftv.unsubst Awf
+a ∈ ftv(A)
+────────────── typeAppr
+a ∈ ftv(E [A])
 
-theorem NotInFreeTermVars'Types'FreeTypeVars.appl (anin : [[G ⊢ a ∉ fvftv(E F)]])
-  : [[G ⊢ a ∉ fvftv(E)]] := by
-  intro ain
-  apply anin
-  let .mk x'infv x'A'inG ainftv := ain
-  exact .mk x'infv.appl x'A'inG ainftv
+namespace InTermFreeTypeVars
 
-theorem NotInFreeTermVars'Types'FreeTypeVars.appr (anin : [[G ⊢ a ∉ fvftv(E F)]])
-  : [[G ⊢ a ∉ fvftv(F)]] := by
-  intro ain
-  apply anin
-  let .mk x'infv x'A'inG ainftv := ain
-  exact .mk x'infv.appr x'A'inG ainftv
+theorem of_TermVar_open {E : Term} : InTermFreeTypeVars a (E.TermVar_open x n) → [[a ∈ ftv(E)]] :=
+  fun ainEop => by
+  match E with
+  | .var _ => nomatch ainEop
+  | .lam A E' =>
+    rw [Term.TermVar_open] at ainEop
+    match ainEop with
+    | .laml ainA => exact .laml ainA
+    | .lamr ainE' => exact .lamr ainE'.of_TermVar_open
+  | .app E' F =>
+    rw [Term.TermVar_open] at ainEop
+    match ainEop with
+    | .appl ainE' => exact .appl ainE'.of_TermVar_open
+    | .appr ainF => exact .appr ainF.of_TermVar_open
+  | .typeGen E' =>
+    rw [Term.TermVar_open] at ainEop
+    let .typeGen ainE' := ainEop
+    exact .typeGen ainE'.of_TermVar_open
+  | .typeApp E' A =>
+    rw [Term.TermVar_open] at ainEop
+    match ainEop with
+    | .typeAppl ainE' => exact .typeAppl ainE'.of_TermVar_open
+    | .typeAppr ainA => exact .typeAppr ainA
 
-theorem NotInFreeTermVars'Types'FreeTypeVars.typeGen (anin : [[G ⊢ a ∉ fvftv(Λ b. E)]])
-  : [[G ⊢ a ∉ fvftv(E)]] := by
-  intro ain
-  apply anin
-  let .mk x'infv x'A'inG ainftv := ain
-  exact .mk x'infv.typeGen x'A'inG ainftv
+theorem of_TypeVar_open {E : Term} (h : a ≠ a')
+  : InTermFreeTypeVars a (E.TypeVar_open a' n) → [[a ∈ ftv(E)]] := fun ainEop => by
+  match E with
+  | .var _ => nomatch ainEop
+  | .lam A E' =>
+    rw [Term.TypeVar_open] at ainEop
+    match ainEop with
+    | .laml ainA => exact .laml <| ainA.of_TypeVar_open h
+    | .lamr ainE' => exact .lamr <| ainE'.of_TypeVar_open h
+  | .app E' F =>
+    rw [Term.TypeVar_open] at ainEop
+    match ainEop with
+    | .appl ainE' => exact .appl <| ainE'.of_TypeVar_open h
+    | .appr ainF => exact .appr <| ainF.of_TypeVar_open h
+  | .typeGen E' =>
+    rw [Term.TypeVar_open] at ainEop
+    let .typeGen ainE' := ainEop
+    exact .typeGen <| ainE'.of_TypeVar_open h
+  | .typeApp E' A =>
+    rw [Term.TypeVar_open] at ainEop
+    match ainEop with
+    | .typeAppl ainE' => exact .typeAppl <| ainE'.of_TypeVar_open h
+    | .typeAppr ainA => exact .typeAppr <| ainA.of_TypeVar_open h
 
-theorem NotInFreeTermVars'Types'FreeTypeVars.typeApp (anin : [[G ⊢ a ∉ fvftv(E [A])]])
-  : [[G ⊢ a ∉ fvftv(E)]] := by
-  intro ain
-  apply anin
-  let .mk x'infv x'A'inG ainftv := ain
-  exact .mk x'infv.typeApp x'A'inG ainftv
+theorem exists_gt (E : Term) : ∃ a : Nat, ∀ a' : Nat, [[a' ∈ ftv(E)]] → a' < a :=
+  match E with
+  | .var _ => .intro 0 fun _ x'in => nomatch x'in
+  | .lam A E' =>
+    let ⟨aA, aAgt⟩ := InTypeFreeTypeVars.exists_gt A
+    let ⟨aE', aE'gt⟩ := exists_gt E'
+    .intro (max aA aE') fun
+      | _, .laml a'infvA =>
+        Nat.lt_of_lt_of_le (aAgt _ a'infvA) <| Nat.le_max_left _ _
+      | _, .lamr a'infvE' =>
+        Nat.lt_of_lt_of_le (aE'gt _ a'infvE') <| Nat.le_max_right _ _
+  | .app E' F =>
+    let ⟨aE', aE'gt⟩ := exists_gt E'
+    let ⟨aF, aFgt⟩ := exists_gt F
+    .intro (max aE' aF) fun
+      | _, .appl a'infvE' =>
+        Nat.lt_of_lt_of_le (aE'gt _ a'infvE') <| Nat.le_max_left _ _
+      | _, .appr a'infvF =>
+        Nat.lt_of_lt_of_le (aFgt _ a'infvF) <| Nat.le_max_right _ _
+  | .typeGen E' =>
+    let ⟨aE', aE'gt⟩ := exists_gt E'
+    .intro aE' fun | _, .typeGen a'infvE' => aE'gt _ a'infvE'
+  | .typeApp E' A =>
+    let ⟨aE', aE'gt⟩ := exists_gt E'
+    let ⟨aA, aAgt⟩ := InTypeFreeTypeVars.exists_gt A
+    .intro (max aE' aA) fun
+      | _, .typeAppl a'infvE' =>
+        Nat.lt_of_lt_of_le (aE'gt _ a'infvE') <| Nat.le_max_left _ _
+      | _, .typeAppr a'infvA =>
+        Nat.lt_of_lt_of_le (aAgt _ a'infvA) <| Nat.le_max_right _ _
+
+end InTermFreeTypeVars
+
+judgement_syntax a " ∉ " "ftv" "(" E ")" : NotInTermFreeTypeVars (id a)
+
+def NotInTermFreeTypeVars a E := ¬[[a ∈ ftv(E)]]
+
+namespace NotInTermFreeTypeVars
+
+theorem lam : [[a ∉ ftv(λ x : A. E)]] → [[a ∉ ftv(A)]] ∧ [[a ∉ ftv(E)]] :=
+  fun anin => ⟨(anin <| .laml ·), (anin <| .lamr ·)⟩
+
+theorem app : [[a ∉ ftv(E F)]] → [[a ∉ ftv(E)]] ∧ [[a ∉ ftv(F)]] :=
+  fun anin => ⟨(anin <| .appl ·), (anin <| .appr ·)⟩
+
+theorem typeGen : [[a ∉ ftv(Λ a. E)]] → [[a ∉ ftv(E)]] := (· <| .typeGen ·)
+
+theorem typeApp : [[a ∉ ftv(E [A])]] → [[a ∉ ftv(E)]] ∧ [[a ∉ ftv(A)]] :=
+  fun anin => ⟨(anin <| .typeAppl ·), (anin <| .typeAppr ·)⟩
+
+theorem TermVar_open : [[a ∉ ftv(E)]] → [[a ∉ ftv(E^x)]] := (· <| ·.of_TermVar_open)
+
+theorem TypeVar_open_of_ne (h : a ≠ a') : [[a ∉ ftv(E)]] → [[a ∉ ftv(E^a')]] :=
+  (· <| ·.of_TypeVar_open h)
+
+theorem exists_fresh {I : List _} : ∃ a ∉ I, [[a ∉ ftv(E)]] ∧ [[a ∉ ftv(A)]] :=
+  let ⟨aI, aIgt⟩ := I.exists_gt
+  let ⟨aE, aEgt⟩ := InTermFreeTypeVars.exists_gt E
+  let ⟨aA, aAgt⟩ := InTypeFreeTypeVars.exists_gt A
+  .intro (max aI (max aE aA) : Nat) ⟨
+    fun inI => Nat.not_le_of_lt (aIgt _ inI) <| Nat.le_max_left _ _,
+    fun inE => Nat.not_le_of_lt (aEgt _ inE) <|
+      Nat.le_trans (Nat.le_max_left _ _) <| Nat.le_max_right _ _,
+    fun inA => Nat.not_le_of_lt (aAgt _ inA) <|
+      Nat.le_trans (Nat.le_max_right _ _) <| Nat.le_max_right _ _
+  ⟩
+
+end NotInTermFreeTypeVars
+
+judgement_syntax G " ⊢ " A : TypeWellFormedness
+
+judgement TypeWellFormedness :=
+
+a ∈ G
+───── var
+G ⊢ a
+
+G ⊢ A
+G ⊢ B
+───────── arr
+G ⊢ A → B
+
+∀ a ∉ (I : List _), G, a ⊢ A^a
+────────────────────────────── forall'
+G ⊢ ∀ a. A
+
+namespace TypeWellFormedness
+
+theorem TermVar_drop (Bwf : [[G, x : A, G' ⊢ B]]) : [[G, G' ⊢ B]] :=
+  match B, Bwf with
+  | .var _, var ainGxAGG => match ainGxAGG.append_elim with
+    | .inl (.termVarExt ainG) => var ainG.append_inl
+    | .inr ainGG => var ainGG.append_inr
+  | .arr .., arr A'wf B'wf => arr A'wf.TermVar_drop B'wf.TermVar_drop
+  | .forall' _, forall' A'wf => forall' fun a anin => by
+    have := A'wf a anin
+    rw [← Environment.append_typeVarExt] at this
+    exact this.TermVar_drop
+
+theorem weakening (Awf : [[G ⊢ A]]) : [[G', G ⊢ A]] := match Awf with
+  | var ain => var ain.append_inr
+  | arr A'wf Bwf => arr A'wf.weakening Bwf.weakening
+  | forall' (I := I) A'wf => forall' (I := I) fun a anin => A'wf a anin |>.weakening
+
+theorem TypeVarLocallyClosed_of : [[G ⊢ A]] → A.TypeVarLocallyClosed G.typeVar_count :=
+  fun Awf =>
+  match A, Awf with
+  | _, .var _ => .var_free
+  | .arr _ _, .arr A'wf Bwf => .arr A'wf.TypeVarLocallyClosed_of Bwf.TypeVarLocallyClosed_of
+  | .forall' A', .forall' A'wf (I := I) => by
+    let ⟨a, anin⟩ := I.exists_fresh
+    have := A'wf a anin |>.TypeVarLocallyClosed_of
+    rw [Environment.typeVar_count, Nat.add_comm] at this
+    exact .forall' <| this.TypeVar_open_drop <| Nat.zero_lt_succ _
+
+theorem TypeVarLocallyClosed_of_empty : [[ε ⊢ A]] → A.TypeVarLocallyClosed 0 :=
+  TypeVarLocallyClosed_of
+
+theorem Type'_open_preservation {A : Type'} {G : Environment} (aninftvA : [[a ∉ ftv(A)]]) (Bwf : [[ε ⊢ B]])
+  : TypeWellFormedness ((Environment.empty.typeVarExt a).append (G.TypeVar_open a n))
+    (A.TypeVar_open a n) →
+    TypeWellFormedness (G.Type'_open B n) (A.Type'_open B n) := fun Aopwf => by
+  match A with
+  | .var (.free a') =>
+    rw [Type'.TypeVar_open, if_neg (nomatch ·)] at Aopwf
+    let .var a'inaG := Aopwf
+    match a'inaG.append_elim with
+    | .inl .head => exact aninftvA .var |>.elim
+    | .inr a'inG => exact .var a'inG.Type'_open
+  | .var (.bound _) =>
+    rw [Type'.Type'_open]
+    split
+    · case isTrue h => exact Bwf.weakening
+    · case isFalse h =>
+      rw [Type'.TypeVar_open, if_neg h] at Aopwf
+      nomatch Aopwf
+  | .arr A' B' =>
+    rw [Type'.TypeVar_open] at Aopwf
+    let .arr A'wf B'wf := Aopwf
+    exact .arr (Type'_open_preservation (NotInTypeFreeTypeVars.arr.mp aninftvA).left Bwf A'wf)
+      (Type'_open_preservation (NotInTypeFreeTypeVars.arr.mp aninftvA).right Bwf B'wf)
+  | .forall' A' =>
+    rw [Type'.TypeVar_open] at Aopwf
+    simp only at Aopwf
+    let .forall' A'wf (I := I) := Aopwf
+    exact .forall' (I := a :: I) <| fun a' a'nin => by
+      have a'nea := List.ne_of_not_mem_cons a'nin
+      have := A'wf a' <| List.not_mem_of_not_mem_cons a'nin
+      have Gopeq : (G.TypeVar_open a n).typeVarExt a' = (G.typeVarExt a').TypeVar_open a (n + 1) :=
+        by rw [Environment.TypeVar_open]
+      rw [← A'.TypeVar_open_Type'_open_eq Bwf.TypeVarLocallyClosed_of_empty (Nat.zero_ne_add_one _)]
+      rw [A'.TypeVar_open_comm a'nea.symm (Nat.succ_ne_zero _), ← Environment.append_typeVarExt,
+          Gopeq] at this
+      exact Type'_open_preservation (aninftvA.forall'.TypeVar_open_of_ne a'nea.symm) Bwf this
+
+end TypeWellFormedness
 
 judgement_syntax G " ⊢ " E " : " A : Typing
 
@@ -797,8 +1511,8 @@ x : A ∈ G
 G ⊢ x : A
 
 G ⊢ A
-G, x : A ⊢ E : B
-────────────────────── lam
+∀ x ∉ (I : List _), G, x : A ⊢ E^x : B
+────────────────────────────────────── lam
 G ⊢ λ x : A. E : A → B
 
 G ⊢ E : A → B
@@ -806,324 +1520,175 @@ G ⊢ F : A
 ───────────── app
 G ⊢ E F : B
 
-G ⊢ a ∉ fvftv(E)
-G, a ⊢ E : A
-─────────────────── typeGen
+∀ a ∉ (I : List _), G, a ⊢ E^a : A^a
+──────────────────────────────────── typeGen
 G ⊢ Λ a. E : ∀ a. A
 
 G ⊢ E : ∀ a. A
 G ⊢ B
-───────────────────── typeApp
-G ⊢ E [B] : A [B / a]
+──────────────── typeApp
+G ⊢ E [B] : A^^B
 
-theorem Typing.TermVar_swap (EtyB : [[G, y : A', x : A, GG ⊢ E : B]]) (xney : x ≠ y)
-  : [[G, x : A, y : A', GG ⊢ E : B]] :=
-  match EtyB with
-  | .var x'BinGyxappGG =>
-    match x'BinGyxappGG.append_elim with
-    | .inl ⟨x'BinGyx, x'ninGG⟩ => match x'BinGyx with
-      | .head => .var <| TermVarInEnvironment.append_inl (.termVarExt .head xney) x'ninGG
-      | .termVarExt x'BinGy x'nex => match x'BinGy with
-        | .head => .var <| .append_inl .head x'ninGG
-        | .termVarExt x'BinG x'ney =>
-          .var <| x'BinG.termVarExt x'nex |>.termVarExt x'ney |>.append_inl x'ninGG
-    | .inr x'BinGG => .var x'BinGG.append_inr
-  | .lam A'wf E'tyB' =>
-    .lam A'wf.TermVar_swap <| E'tyB'.TermVar_swap (GG := GG.termVarExt ..) xney
-  | .app E'tyA'arrB F'tyA' => .app (E'tyA'arrB.TermVar_swap xney) (F'tyA'.TermVar_swap xney)
-  | .typeGen a'nin E'tyA' =>
-    .typeGen (a'nin.TermVar_swap xney) <| E'tyA'.TermVar_swap (GG := GG.typeVarExt _) xney
-  | .typeApp E'ty B'wf => .typeApp (E'ty.TermVar_swap xney) B'wf.TermVar_swap
+namespace Typing
 
-theorem Typing.False_of_in_fv_of_nin_Environment (EtyA : [[G ⊢ E : A]]) (xinfvE : [[x ∈ fv(E)]])
-  (xninG : [[x ∉ G]]) : False :=
-  match EtyA, xinfvE with
-  | .var x'AinG, .var => xninG _ x'AinG
-  | .lam _ E'tyB', .lam xinfvE' xnex' =>
-    E'tyB'.False_of_in_fv_of_nin_Environment xinfvE' (xninG.termVarExt xnex'.symm)
-  | .app E'tyA'arrA F'tyA', .appl xinfvE' =>
-    E'tyA'arrA.False_of_in_fv_of_nin_Environment xinfvE' xninG
-  | .app _ F'tyA', .appr xinfvF' => F'tyA'.False_of_in_fv_of_nin_Environment xinfvF' xninG
-  | .typeGen _ E'tyA', .typeGen xinfvE' =>
-    E'tyA'.False_of_in_fv_of_nin_Environment xinfvE' xninG.typeVarExt
-  | .typeApp E'ty B'wf, .typeApp xinfvE' => E'ty.False_of_in_fv_of_nin_Environment xinfvE' xninG
+theorem TermVarLocallyClosed_of_empty : [[ε ⊢ E : A]] → E.TermVarLocallyClosed 0 := go
+where
+  go {G : Environment} {E : Term} {A : Type'}
+    : [[G ⊢ E : A]] → E.TermVarLocallyClosed G.termVar_count := fun EtyA => match E, EtyA with
+    | _, .var _ => .var_free
+    | .lam A' E', .lam _ E'ty (I := I) => by
+      let ⟨x, xnin⟩ := I.exists_fresh
+      have := go <| E'ty x xnin
+      rw [Environment.termVar_count, Nat.add_comm] at this
+      exact .lam <| this.TermVar_open_drop <| Nat.zero_lt_succ _
+    | .app _ _, .app E'ty Fty => .app (go E'ty) (go Fty)
+    | .typeGen E', .typeGen E'ty (I := I) => by
+      let ⟨a, anin⟩ := I.exists_fresh
+      exact .typeGen <| go (E'ty a anin) |>.TypeVar_open_drop
+    | .typeApp E' _, .typeApp E'ty _ => .typeApp <| go E'ty
 
-theorem NotInFreeTermVars'Types'FreeTypeVars.append_inr (anin : [[G ⊢ a ∉ fvftv(E)]])
-  (EtyA : [[G, b ⊢ E : A]]) : [[GG, G ⊢ a ∉ fvftv(E)]] := fun ain =>
-  anin <|
-    let .mk x'infv x'A'inGGappG ainftv := ain
-    match x'A'inGGappG.append_elim with
-    | .inl ⟨_, x'ninG⟩ =>
-      False.elim <| EtyA.False_of_in_fv_of_nin_Environment x'infv x'ninG.typeVarExt
-    | .inr x'A'inG => .mk x'infv x'A'inG ainftv
+theorem TypeVarLocallyClosed_of_empty : [[ε ⊢ E : A]] → E.TypeVarLocallyClosed 0 := go
+where
+  go {G : Environment} {E : Term} {A : Type'}
+    : [[G ⊢ E : A]] → E.TypeVarLocallyClosed G.typeVar_count := fun EtyA => match E, EtyA with
+    | _, .var _ => .var
+    | .lam A' E', .lam A'ty E'ty (I := I) => by
+      let ⟨x, xnin⟩ := I.exists_fresh
+      have := go <| E'ty x xnin
+      rw [Environment.typeVar_count] at this
+      exact .lam A'ty.TypeVarLocallyClosed_of this.TermVar_open_drop
+    | .app _ _, .app E'ty Fty => .app (go E'ty) (go Fty)
+    | .typeGen E', .typeGen E'ty (I := I) => by
+      let ⟨a, anin⟩ := I.exists_fresh
+      have := go <| E'ty a anin
+      rw [Environment.typeVar_count, Nat.add_comm] at this
+      apply Term.TypeVarLocallyClosed.typeGen
+      exact this.TypeVar_open_drop <| Nat.zero_lt_succ _
+    | .typeApp E' A', .typeApp E'ty A'ty => .typeApp (go E'ty) A'ty.TypeVarLocallyClosed_of
 
-theorem Typing.append_inr : [[G ⊢ E : A]] → [[GG, G ⊢ E : A]]
-  | .var xAinG => .var xAinG.append_inr
-  | .lam A'wf E'tyB => .lam A'wf.append_inr E'tyB.append_inr
-  | .app FtyA' E'tyA'arrA => .app FtyA'.append_inr E'tyA'arrA.append_inr
-  | .typeGen a'nin E'tyA' => .typeGen (a'nin.append_inr E'tyA') E'tyA'.append_inr
-  | .typeApp E'ty Bwf => .typeApp E'ty.append_inr Bwf.append_inr
+theorem weakening (EtyA : [[G ⊢ E : A]]) : [[G', G ⊢ E : A]] := by
+  induction EtyA with
+  | var xin => exact .var xin.append_inr
+  | lam Awf _ ih => exact .lam Awf.weakening ih
+  | app _ _ ihE ihF => exact .app ihE ihF
+  | typeGen _ ih => exact .typeGen ih
+  | typeApp _ Bwf ih => exact .typeApp ih Bwf.weakening
 
-theorem Typing.TermVar_shadowed : [[G, x : A_shadowed, GG, x : A, GGG ⊢ E : B]] → [[G, GG, x : A, GGG ⊢ E : B]]
-  | var x'BinGxGGxGGG =>
-    match x'BinGxGGxGGG.append_elim with
-    | .inl ⟨x'BinGx, x'ninGGxGGG⟩ =>
-      match x'BinGx with
-      | .head => False.elim <| x'ninGGxGGG A <| TermVarInEnvironment.append_inl .head
-          fun A' xA'inGGG => x'ninGGxGGG A' xA'inGGG.append_inr
-      | .termVarExt x'BinG _ => .var <| x'BinG.append_inl x'ninGGxGGG
-    | .inr x'BinGGxGGG => .var x'BinGGxGGG.append_inr
-  | lam A'wf E'tyB' => .lam A'wf.TermVar_drop <| E'tyB'.TermVar_shadowed (GGG := GGG.termVarExt ..)
-  | app E'tyA'arrB FtyA' => .app E'tyA'arrB.TermVar_shadowed FtyA'.TermVar_shadowed
-  | typeGen a'nin E'tyA' => .typeGen a'nin.TermVar_shadowed <| E'tyA'.TermVar_shadowed (GGG := GGG.typeVarExt _)
-  | typeApp E'ty B'wf => .typeApp E'ty.TermVar_shadowed B'wf.TermVar_drop
-
-theorem Typing.TypeVar_shadowed_subst (EtyA : [[ε, a, G, a, GG ⊢ E : A]]) (Bwf : [[ε ⊢ B]])
-  (aninG : [[a ∉ G]])
-  (ih : ∀ x : TermVar, [[x ∈ fv(E)]] → (∃ A, [[x : A ∈ GG]]) ∨ ∀ A, [[x : A ∈ G]] → [[a ∉ ftv(A)]])
-  : [[(G, a) [B / a], GG ⊢ E : A]] := by
-  cases EtyA
-  · case var x xAinεaGaGG =>
-    match xAinεaGaGG.append_elim with
-    | .inl ⟨xAinεa, _⟩ =>
-      cases xAinεa
-      case typeVarExt xAinε =>
-      cases xAinε
-    | .inr xAinGaGG => match xAinGaGG.append_elim with
-      | .inl ⟨xAinGa, xninGG⟩ =>
-        apply Typing.var
-        apply TermVarInEnvironment.append_inl _ xninGG
-        rw [← Environment.subst_typeVarExt_eq_typeVarExt_subst]
-        apply TermVarInEnvironment.typeVarExt
-        cases xAinGa
-        case a.typeVarExt xAinG =>
-        have aninftvA : [[a ∉ ftv(A)]] := by
-          match ih x .var with
-          | .inl ⟨A', xA'inGG⟩ => exact False.elim <| xninGG A' xA'inGG
-          | .inr h => exact h A xAinG
-        rw [← NotInFreeTypeVars.subst_id aninftvA]
-        exact xAinG.subst aninG
-      | .inr xAinGG => exact .var xAinGG.append_inr
-  · case lam A' x E' B' A'wf E'tyB' =>
-    apply Typing.lam A'wf.TypeVar_shadowed_subst
-    apply E'tyB'.TypeVar_shadowed_subst (GG := GG.termVarExt x A') Bwf aninG
-    intro x' x'infvE'
-    by_cases x' = x
-    · case pos x'eqx =>
-      rw [x'eqx]
-      exact .inl <| Exists.intro A' .head
-    · case neg x'nex =>
-      match ih x' (x'infvE'.lam x'nex) with
-      | .inl ⟨A'', x'A''inGG⟩ => exact .inl <| Exists.intro A'' <| x'A''inGG.termVarExt x'nex
-      | .inr h => exact .inr h
-  · case app E' A' F FtyA' E'tyA'arrA =>
-    exact .app (E'tyA'arrA.TypeVar_shadowed_subst Bwf aninG (ih · ·.appl))
-      (FtyA'.TypeVar_shadowed_subst Bwf aninG (ih · ·.appr))
-  · case typeGen a' E' A' a'nin E'tyA' =>
-    apply Typing.typeGen _ <| E'tyA'.TypeVar_shadowed_subst (GG := GG.typeVarExt a') Bwf aninG _
-    · intro a'in
-      apply a'nin
-      let .mk x'infv x'A'in a'inftv := a'in
-      match x'A'in.append_elim with
-      | .inl ⟨.typeVarExt x'A'in, x'ninGG⟩ =>
-        let ⟨A'', ⟨x'A''in, eq⟩⟩ := x'A'in.unsubst aninG
-        rw [eq] at a'inftv
-        exact .mk x'infv (x'A''in.typeVarExt.append_inl x'ninGG).append_inr <| a'inftv.unsubst Bwf
-      | .inr x'A'inGG => exact .mk x'infv x'A'inGG.append_inr.append_inr a'inftv
-    · intro x xinfvE'
-      match ih x xinfvE'.typeGen with
-      | .inl ⟨A'', x'A''inGG⟩ => exact .inl <| Exists.intro A'' <| x'A''inGG.typeVarExt
-      | .inr h => exact .inr h
-  · case typeApp E' a' A' B' E'ty B'wf =>
-    exact .typeApp (E'ty.TypeVar_shadowed_subst Bwf aninG (ih · ·.typeApp)) B'wf.TypeVar_shadowed_subst
-
-theorem NotInFreeTermVars.of_Typing_of_TermVarNotInEnvironment (EtyA : [[G ⊢ E : A]])
-  (xninG : [[x ∉ G]]) : [[x ∉ fv(E)]] := by
-  intro ain
-  match EtyA, ain with
-  | .var x'inG, .var => exact xninG A x'inG
-  | .lam _ E'tyB, .lam xinE' xnex' =>
-    apply NotInFreeTermVars.of_Typing_of_TermVarNotInEnvironment E'tyB _ xinE'
-    exact xninG.termVarExt xnex'.symm
-  | .app E'tyA'arrA _, .appl xinE' =>
-    exact NotInFreeTermVars.of_Typing_of_TermVarNotInEnvironment E'tyA'arrA xninG xinE'
-  | .app _ F'tyA', .appr xinF' =>
-    exact NotInFreeTermVars.of_Typing_of_TermVarNotInEnvironment F'tyA' xninG xinF'
-  | .typeGen _ E'tyA', .typeGen xinE' =>
-    exact NotInFreeTermVars.of_Typing_of_TermVarNotInEnvironment E'tyA' xninG.typeVarExt xinE'
-  | .typeApp E'ty _, .typeApp xinE' =>
-    exact NotInFreeTermVars.of_Typing_of_TermVarNotInEnvironment E'ty xninG xinE'
-
-theorem InFreeTermVars.unTermVar_subst (xin : [[x ∈ fv(E [F / y])]]) (FtyA : [[ε ⊢ F : A]])
-  : [[x ∈ fv(E)]] := by
+theorem Term_open_preservation {E : Term}
+  (EtyB : Typing ((Environment.empty.termVarExt x A).append G) (E.TermVar_open x n) B)
+  (xninG : [[x ∉ G]]) (xninfvE : [[x ∉ fv(E)]]) (FtyA : [[ε ⊢ F : A]])
+  : Typing G (E.Term_open F n) B := by
   match E with
-  | .var x' =>
-    rw [Term.TermVar_subst] at xin
-    split at xin
-    · case isTrue x'eqx =>
-      exact False.elim <|
-        NotInFreeTermVars.of_Typing_of_TermVarNotInEnvironment FtyA TermVarNotInEnvironment.ε xin
-    · case isFalse x'nex =>
-      let .var := xin
-      exact .var
-  | .lam x' A' E' =>
-    rw [Term.TermVar_subst] at xin
-    split at xin
-    · case isTrue x'eqy => exact xin
-    · case isFalse x'ney =>
-      let .lam xinE' xnex' := xin
-      exact .lam (xinE'.unTermVar_subst FtyA) xnex'
-  | .app E' F' =>
-    rw [Term.TermVar_subst] at xin
-    match xin with
-    | .appl xinE' => exact .appl <| xinE'.unTermVar_subst FtyA
-    | .appr xinF' => exact .appr <| xinF'.unTermVar_subst FtyA
-  | .typeGen a' E' =>
-    rw [Term.TermVar_subst] at xin
-    let .typeGen xinE' := xin
-    exact .typeGen <| xinE'.unTermVar_subst FtyA
-  | .typeApp E' A'' =>
-    rw [Term.TermVar_subst] at xin
-    let .typeApp xinE' := xin
-    exact .typeApp <| xinE'.unTermVar_subst FtyA
-
-theorem NotInFreeTermVars'Types'FreeTypeVars.Term_TermVar_subst (anin : [[G ⊢ a ∉ fvftv(E)]])
-  (FtyA : [[ε ⊢ F : A]]) : [[G ⊢ a ∉ fvftv(E [F / x])]] := by
-  intro ain
-  apply anin
-  cases ain
-  case mk x' A' x'A'inG ainftv x'infv =>
-  exact InFreeTermVars'Types'FreeTypeVars.mk (x'infv.unTermVar_subst FtyA) x'A'inG ainftv
-
-theorem InFreeTermVars.unTypeVar_subst (xin : [[x ∈ fv(E [B / b])]]) : [[x ∈ fv(E)]] := by
-  match E with
-  | .var x' =>
-    rw [Term.TypeVar_subst] at xin
-    exact xin
-  | .lam x' A' E' =>
-    rw [Term.TypeVar_subst] at xin
-    let .lam xinE' xnex' := xin
-    exact InFreeTermVars.lam xinE'.unTypeVar_subst xnex'
-  | .app E' F' =>
-    rw [Term.TypeVar_subst] at xin
-    match xin with
-    | .appl xinE' => exact .appl xinE'.unTypeVar_subst
-    | .appr xinF' => exact .appr xinF'.unTypeVar_subst
-  | .typeGen a' E' =>
-    rw [Term.TypeVar_subst] at xin
-    split at xin
-    · case isTrue a'eqb => exact xin
-    · case isFalse a'neb =>
-      let .typeGen xinE' := xin
-      exact .typeGen xinE'.unTypeVar_subst
-  | .typeApp E' A'' =>
-    rw [Term.TypeVar_subst] at xin
-    let .typeApp xinE' := xin
-    exact .typeApp xinE'.unTypeVar_subst
-
-theorem NotInFreeTermVars'Types'FreeTypeVars.Term_TypeVar_subst (anin : [[G ⊢ a ∉ fvftv(E)]])
-  : [[G ⊢ a ∉ fvftv(E [A / b])]] := by
-  intro ain
-  apply anin
-  cases ain
-  case mk x' A' x'A'inG ainftv x'infv =>
-  exact InFreeTermVars'Types'FreeTypeVars.mk x'infv.unTypeVar_subst x'A'inG ainftv
-
-theorem Typing.TermVar_subst_preservation (EtyB : [[ε, x : A, G ⊢ E : B]]) (xninG : [[x ∉ G]])
-  (FtyA : [[ε ⊢ F : A]]) : [[G ⊢ E [F / x] : B]] := by
-  match EtyB with
-  | .var x'BinεxappG =>
-    rw [Term.TermVar_subst]
+  | .var (.free _) =>
+    rw [Term.Term_open, if_neg (nomatch ·)]
+    let .var x'BinεxAG := EtyB
+    match x'BinεxAG.append_elim with
+    | .inl ⟨.head, _⟩ => exact xninfvE .var |>.elim
+    | .inr xBinG => exact var xBinG
+  | .var (.bound _) =>
+    rw [Term.Term_open]
     split
-    · case isTrue xeqx' =>
-      rw [← xeqx'] at x'BinεxappG
-      match x'BinεxappG.append_elim with
-      | .inl ⟨xBinεx, _⟩ =>
-        cases xBinεx
-        · case head => exact FtyA.append_inr
-        · case termVarExt xBinε xnex => contradiction
-      | .inr xBinG =>
-        exact False.elim <| xninG B xBinG
-    · case isFalse x'nex =>
-      match x'BinεxappG.append_elim with
-      | .inl ⟨xBinGx, xninG⟩ =>
-        cases xBinGx
-        · case head => contradiction
-        · case termVarExt x'Binε _ => cases x'Binε
-      | .inr x'BinG => exact .var x'BinG
-  | .lam A'wf E'tyB' =>
-    rw [Term.TermVar_subst]
-    split
-    · case isTrue xeqx' =>
-      rw [← xeqx', G.empty_append]
-      rw [← xeqx'] at E'tyB'
-      exact .lam A'wf.TermVar_drop <| E'tyB'.TermVar_shadowed (GGG := .empty)
-    · case isFalse xnex' =>
-      rw [G.empty_append]
-      apply Typing.lam A'wf.TermVar_drop
-      rw [← G.empty_append]
-      apply E'tyB'.TermVar_subst_preservation (G := G.termVarExt ..) _ FtyA
-      have xnex' : x ≠ _ := xnex'
-      exact xninG.termVarExt xnex'.symm
-  | .app E'tyA'arrB F'tyA' =>
-    exact .app (E'tyA'arrB.TermVar_subst_preservation xninG FtyA) (F'tyA'.TermVar_subst_preservation xninG FtyA)
-  | .typeGen a'nin E'tyA' =>
-    apply Typing.typeGen <| a'nin.append_elr.Term_TermVar_subst FtyA
-    apply E'tyA'.TermVar_subst_preservation (G := G.typeVarExt _) _ FtyA
-    exact xninG.typeVarExt
-  | .typeApp E'ty B'wf =>
-    apply Typing.typeApp <| E'ty.TermVar_subst_preservation xninG FtyA
-    rw [G.empty_append]
-    exact B'wf.TermVar_drop
+    · case isTrue h =>
+      rw [← h, Term.TermVar_open, if_pos rfl] at EtyB
+      let .var xBinxAG := EtyB
+      match xBinxAG.append_elim with
+      | .inl ⟨.head, _⟩ => exact FtyA.weakening
+      | .inr xBinG => exact xninG _ xBinG |>.elim
+    · case isFalse h =>
+      rw [Term.TermVar_open, if_neg h] at EtyB
+      nomatch EtyB
+  | .lam A' E' =>
+    rw [Term.Term_open]
+    simp only
+    let .lam A'wf E'ty (I := I) := EtyB
+    rw [← G.empty_append]
+    exact lam (I := x :: I) A'wf.TermVar_drop fun x' x'nin => by
+      have x'nex := List.ne_of_not_mem_cons x'nin
+      have := E'ty x' <| List.not_mem_of_not_mem_cons x'nin
+      rw [Environment.empty_append,
+          ← E'.TermVar_open_Term_open_eq (n := n + 1) (m := 0)
+            FtyA.TermVarLocallyClosed_of_empty (Nat.zero_ne_add_one _)]
+      rw [← Environment.append_termVarExt,
+          E'.TermVar_open_comm x'nex.symm (Nat.succ_ne_zero _)] at this
+      exact this.Term_open_preservation (xninG.termVarExt x'nex.symm)
+        (xninfvE.lam.TermVar_open_of_ne x'nex.symm) FtyA
+  | .app E' F =>
+    let .app E'ty Fty := EtyB
+    rw [Term.Term_open]
+    exact app (E'ty.Term_open_preservation xninG xninfvE.app.left FtyA)
+      (Fty.Term_open_preservation xninG xninfvE.app.right FtyA)
+  | .typeGen E' =>
+    let .typeGen E'ty := EtyB
+    rw [Term.Term_open]
+    exact typeGen fun a anin => by
+      have := E'ty a anin
+      rw [← E'.TypeVar_open_Term_open_eq FtyA.TypeVarLocallyClosed_of_empty]
+      rw [← Environment.append_typeVarExt, E'.TermVar_open_TypeVar_open_eq] at this
+      exact this.Term_open_preservation xninG.typeVarExt
+        xninfvE.typeGen.TypeVar_open FtyA
+  | .typeApp E' A' =>
+    let .typeApp E'ty A'wf := EtyB
+    have := A'wf.TermVar_drop
+    rw [G.empty_append] at this
+    exact typeApp (E'ty.Term_open_preservation xninG xninfvE.typeApp FtyA) this
 
-theorem Typing.TypeVar_subst_preservation (EtyA : [[ε, a, G ⊢ E : A]]) (aninG : [[a ∉ G]])
-  (Bwf : [[ε ⊢ B]]) : [[G [B / a] ⊢ E [B / a] : A [B / a] ]] := by
-  cases EtyA
-  · case var x xAinεaappG => match xAinεaappG.append_elim with
-    | .inr xAinG => exact .var <| xAinG.subst aninG
-  · case lam A' x E' B' A'wf E'tyB' =>
-    rw [Term.TypeVar_subst]
-    rw [← Environment.append] at E'tyB'
-    apply Typing.lam (A'wf.subst Bwf)
-    rw [Environment.subst_termVarExt_eq_termVarExt_subst_of_TypeVarNotInEnvironment aninG]
-    exact E'tyB'.TypeVar_subst_preservation (G := G.termVarExt x A') aninG.termVarExt Bwf
-  · case app E' A' F FtyA' E'tyA'arrA =>
-    exact .app (E'tyA'arrA.TypeVar_subst_preservation aninG Bwf) (FtyA'.TypeVar_subst_preservation aninG Bwf)
-  · case typeGen a' E' A' a'nin E'tyA' =>
-    rw [Term.TypeVar_subst]
-    split
-    · case isTrue aeqa' =>
-      rw [← aeqa', ← Type'.subst_shadowed_forall]
-      rw [← aeqa'] at E'tyA' a'nin
-      apply Typing.typeGen <| a'nin.append_elr.Environment_subst Bwf aninG
-      rw [Environment.subst_typeVarExt_eq_typeVarExt_subst]
-      apply E'tyA'.TypeVar_shadowed_subst (GG := .empty) Bwf aninG
-      intro x xinfvE'
-      right
-      intro A'' xA''inG ainftvA''
-      exact a'nin <| InFreeTermVars'Types'FreeTypeVars.mk xinfvE' xA''inG.append_inr ainftvA''
-    · case isFalse anea' =>
-      rw [Type'.TypeVar_subst, if_neg anea']
-      apply Typing.typeGen <| a'nin.append_elr.Term_TypeVar_subst.Environment_subst Bwf aninG
-      rw [Environment.subst_typeVarExt_eq_typeVarExt_subst]
-      have anea' : a ≠ a' := anea'
-      exact E'tyA'.TypeVar_subst_preservation (G := G.typeVarExt a') (aninG.typeVarExt anea'.symm) Bwf
-  · case typeApp E' a' A' B' E'ty B'wf =>
-    rw [Term.TypeVar_subst]
-    by_cases a' = a
-    · case pos a'eqa =>
-      rw [a'eqa, Type'.subst_subst]
-      rw [a'eqa] at E'ty
-      apply Typing.typeApp _ (B'wf.subst Bwf)
-      rw [Type'.subst_shadowed_forall B]
-      exact E'ty.TypeVar_subst_preservation aninG Bwf
-    · case neg a'nea =>
-      -- TODO: Probably need to use alpha equivalence to avoid issues when B' contains a.
-      have : ((A'.TypeVar_subst a' B').TypeVar_subst a B) = (A'.TypeVar_subst a B).TypeVar_subst a' (B'.TypeVar_subst a B) := sorry
-      rw [this]
-      apply Typing.typeApp _ <| B'wf.subst Bwf
-      rw [Type'.forall_subst_eq_subst_forall a'nea]
-      exact E'ty.TypeVar_subst_preservation aninG Bwf
+theorem Type'_open_preservation {E : Term} {A : Type'}
+  (EtyA : Typing ((Environment.empty.typeVarExt a).append (G.TypeVar_open a n))
+    (E.TypeVar_open a n) (A.TypeVar_open a n)) (aninG : [[a ∉ G]]) (aninftvE : [[a ∉ ftv(E)]])
+  (aninftvA : [[a ∉ ftv(A)]]) (Bwf : [[ε ⊢ B]])
+  : Typing (G.Type'_open B n) (E.Type'_open B n) (A.Type'_open B n) := by
+  generalize E'eq : E.TypeVar_open a n = E', A'eq : A.TypeVar_open a n = A' at *
+  match E, A, EtyA with
+  | .var (.free x), A, .var xAopinεaG =>
+    rw [Term.Type'_open]
+    cases E'eq
+    cases A'eq
+    let .inr xAopinG := xAopinεaG.append_elim
+    exact var xAopinG.Type'_open
+  | .lam A'' E'', .arr A''' B', .lam A''wf E''ty (A := A'''') (B := B'') =>
+    rw [Term.Type'_open, Type'.Type'_open]
+    cases E'eq
+    rw [Type'.TypeVar_open] at A'eq
+    let ⟨A''opeq, B'opeq⟩ := Type'.arr.inj A'eq
+    cases B'opeq
+    cases NotInTypeFreeTypeVars.TypeVar_open_inj_of (NotInTypeFreeTypeVars.arr.mp aninftvA).left
+      aninftvE.lam.left A''opeq
+    exact Typing.lam (TypeWellFormedness.Type'_open_preservation aninftvE.lam.left Bwf A''wf)
+      fun x' x'nin => by
+        have := E''ty x' x'nin
+        rw [← Environment.Type'_open, ← E''.TermVar_open_Type'_open_comm]
+        rw [← Environment.append_termVarExt, ← Term.TermVar_open_TypeVar_open_eq] at this
+        exact this.Type'_open_preservation aninG.termVarExt aninftvE.lam.right.TermVar_open
+          (NotInTypeFreeTypeVars.arr.mp aninftvA).right Bwf
+  | .app E'' F, A, .app E''ty Fty (A := A'') =>
+    rw [Term.Type'_open]
+    cases E'eq
+    cases A'eq
+    sorry
+  | .typeGen E', .forall' A', .typeGen E'ty (I := I) =>
+    cases E'eq
+    cases A'eq
+    exact .typeGen (I := a :: I) fun a' a'nin => by
+      have a'nea := List.ne_of_not_mem_cons a'nin
+      have := E'ty a' <| List.not_mem_of_not_mem_cons a'nin
+      rw [← E'.TypeVar_open_Type'_open_eq Bwf.TypeVarLocallyClosed_of_empty (Nat.zero_ne_add_one _),
+          ← A'.TypeVar_open_Type'_open_eq Bwf.TypeVarLocallyClosed_of_empty (Nat.zero_ne_add_one _)]
+      have Gopeq : (G.TypeVar_open a n).typeVarExt a' = (G.typeVarExt a').TypeVar_open a (n + 1) :=
+        by rw [Environment.TypeVar_open]
+      rw [← Environment.append_typeVarExt, E'.TypeVar_open_comm a'nea.symm (Nat.succ_ne_zero _),
+          A'.TypeVar_open_comm a'nea.symm (Nat.succ_ne_zero _), Gopeq] at this
+      exact this.Type'_open_preservation (G := G.typeVarExt a')
+        (aninG.typeVarExt a'nea.symm)
+        (aninftvE.typeGen.TypeVar_open_of_ne a'nea.symm)
+        (aninftvA.forall'.TypeVar_open_of_ne a'nea.symm) Bwf
+  | .typeApp E' B', A, .typeApp E'ty B'wf (A := A') =>
+    rw [Term.Type'_open]
+    cases E'eq
+    sorry
+termination_by sizeOf E
+decreasing_by all_goals sorry
+
+end Typing
 
 judgement_syntax E " -> " F : OperationalSemantics
 
@@ -1137,56 +1702,56 @@ F -> F'
 ─────────── appr
 V F -> V F'
 
-─────────────────────────── lamApp
-(λ x : A. E) V -> E [V / x]
+────────────────────── lamApp
+(λ x : A. E) V -> E^^V
 
 E -> E'
 ─────────────── typeApp
 E [A] -> E' [A]
 
-───────────────────────── typeGenApp
-(Λ a. E) [A] -> E [A / a]
+──────────────────── typeGenApp
+(Λ a. E) [A] -> E^^A
+
+namespace OperationalSemantics
 
 theorem preservation (EtyA : [[ε ⊢ E : A]]) (EstepF : [[E -> F]]) : [[ε ⊢ F : A]] :=
   match EstepF, EtyA with
-  | .appl E'stepE'next, .app E'tyA'arrA FtyA' => .app (preservation E'tyA'arrA E'stepE'next) FtyA'
-  | .appr FstepFnext, .app VtyA'arrA FtyA' => .app VtyA'arrA <| preservation FtyA' FstepFnext
-  | .lamApp, .app (.lam _ E'tyA) VtyA'' =>
-      E'tyA.TermVar_subst_preservation (G := .empty) TermVarNotInEnvironment.ε VtyA''
-  | .typeApp E'stepE'next, .typeApp E'ty A'wf => .typeApp (preservation E'ty E'stepE'next) A'wf
-  | .typeGenApp, .typeApp (.typeGen _ E'tyA'') A'wf =>
-    E'tyA''.TypeVar_subst_preservation (G := .empty) TypeVarNotInEnvironment.ε A'wf
+  | appl E'stepE'next, .app E'tyA'arrA FtyA' =>.app (E'stepE'next.preservation E'tyA'arrA) FtyA'
+  | appr FstepFnext, .app VtyA'arrA FtyA' => .app VtyA'arrA <| FstepFnext.preservation FtyA'
+  | lamApp, .app (.lam _ E'tyA (E := E')) VtyA'' =>
+    let ⟨x, xnin, xninfv⟩ := NotInFreeTermVars.exists_fresh
+    .Term_open_preservation (E'tyA x xnin) (fun _ => (nomatch ·)) xninfv VtyA''
+  | typeApp E'stepE'next, .typeApp E'ty A'wf => .typeApp (E'stepE'next.preservation E'ty) A'wf
+  | typeGenApp, .typeApp (.typeGen E'tyA'') A'wf =>
+    let ⟨a, anin, aninftvE', aninftvA''⟩ := NotInTermFreeTypeVars.exists_fresh
+    .Type'_open_preservation (G := .empty) (E'tyA'' a anin) (nomatch ·) aninftvE' aninftvA'' A'wf
 
 theorem progress (EtyA : [[ε ⊢ E : A]]) : (∃ F, [[E -> F]]) ∨ ∃ V : Value, V.val = E :=
   match E, EtyA with
-  | .lam x A' E', _ =>
-    .inr <| Exists.intro { val := .lam x A' E', property := .lam } rfl
-  | .app E' F', .app E'tyA'arrA F'tyA' =>
-    match progress E'tyA'arrA with
-    | .inl ⟨E'_next, E'stepE'_next⟩ => .inl <| Exists.intro (E'_next.app F') (.appl E'stepE'_next)
+  | .lam .., _ => .inr <| .intro ⟨_, .lam⟩ rfl
+  | .app E' F', .app E'tyA'arrA F'tyA' => match progress E'tyA'arrA with
+    | .inl ⟨E'_next, E'stepE'_next⟩ => .inl <| .intro _ <| appl E'stepE'_next
     | .inr ⟨VE', VE'eqE'⟩ => by
       match progress F'tyA' with
       | .inl ⟨F'_next, F'stepF'_next⟩ =>
         rw [← VE'eqE']
-        exact .inl <| Exists.intro (VE'.val.app F'_next) (.appr F'stepF'_next)
+        exact .inl <| .intro _ <| appr F'stepF'_next
       | .inr ⟨VF', VF'eqF'⟩ =>
         have E'val := VE'.property
         rw [VE'eqE'] at E'val
-        match E' with
-        | .lam x A' E'' =>
-          rw [← VF'eqF']
-          exact .inl <| Exists.intro (E''.TermVar_subst x VF'.val) .lamApp
-  | .typeGen a E', _ =>
-    .inr <| Exists.intro { val := .typeGen a E', property := .typeGen } rfl
-  | .typeApp E' A', .typeApp E'ty A'wf =>
-    match progress E'ty with
-    | .inl ⟨E'_next, E'stepE'_next⟩ =>
-      .inl <| Exists.intro (E'_next.typeApp A') <| .typeApp E'stepE'_next
+        let .lam A' E'' := E'
+        rw [← VF'eqF']
+        exact .inl <| .intro _ lamApp
+  | .typeGen _, _ => .inr <| .intro ⟨_, .typeGen⟩ rfl
+  | .typeApp E' A', .typeApp E'ty _ => match progress E'ty with
+    | .inl ⟨E'_next, E'stepE'_next⟩ => .inl <| .intro _ <| typeApp E'stepE'_next
     | .inr ⟨VE', VE'eqE'⟩ => by
       have E'val := VE'.property
       rw [VE'eqE'] at E'val
-      match E' with
-      | .typeGen a E'' => exact .inl <| Exists.intro (E''.TypeVar_subst a A') .typeGenApp
+      let .typeGen E'' := E'
+      exact .inl <| .intro _ typeGenApp
+
+end OperationalSemantics
 
 filter "LottExamples/SystemF/main.tex" "LottExamples/SystemF/main.mng"
 
