Lott/DSL/Elab/JudgementComprehension.lean
@@ -7,7 +7,7 @@ open Lean.Elab
 
 @[lott_term_elab Lott.DSL.judgementComprehension]
 private
-def judgementComprehensionTermElab : TermElab := fun stx => do
+def judgementComprehensionTermElab : TermElab := fun _ stx => do
   let `(Lott.Judgement| </ $«judgement»:Lott.Judgement // $i ∈ $c />) := stx
     | throwUnsupportedSyntax
   Lean.Elab.Term.elabTerm (← ``(∀ $i:ident ∈ $c, [[$«judgement»:Lott.Judgement]])) none
