Lott/DSL/Elab/UniversalJudgement.lean
@@ -1,0 +1,20 @@
+import Lott.DSL.Elab.Basic
+import Lott.DSL.Parser.UniversalJudgement
+
+namespace Lott.DSL.Elab
+
+open Lean.Elab
+
+@[lott_term_elab Lott.DSL.universalJudgement]
+private
+def universalJudgementTermElab : TermElab := fun _ stx => do
+  let `(Lott.Judgement| ∀ $i $[$binderPred?]?, $«judgement»:Lott.Judgement) := stx
+    | throwUnsupportedSyntax
+  let stx' ← if let some bp := binderPred? then
+      ``(∀ $i:ident, satisfies_binder_pred% $i $bp → [[$«judgement»:Lott.Judgement]])
+    else
+      ``(∀ $i:ident, [[$«judgement»:Lott.Judgement]])
+  Lean.Elab.Term.elabTerm stx' none
+
+end Lott.DSL.Elab
+
