Lott/DSL/Environment/MetaVar.lean
@@ -1,0 +1,16 @@
+import Lean
+
+namespace Lott.DSL
+
+open Lean
+
+initialize metaVarExt : PersistentEnvExtension (Name × Bool) (Name × Bool) (NameMap Bool) ←
+  registerPersistentEnvExtension {
+  mkInitial := return default
+  addImportedFn := fun metaVarss =>
+    return metaVarss.flatten.foldl (init := mkNameMap _) (fun acc (n, ln) => acc.insert n ln)
+  addEntryFn := fun st (n, ln) => st.insert n ln
+  exportEntriesFn := RBMap.fold (cmp := Name.quickCmp) (init := #[]) fun acc n ln => acc.push (n, ln)
+}
+
+end Lott.DSL
