Lott/DSL/Parser/UniversalJudgement.lean
@@ -1,0 +1,7 @@
+import Lott.DSL.Parser
+
+namespace Lott.DSL
+
+syntax (name := universalJudgement) "∀ " ident (binderPred)? ", " withPosition(Lott.Judgement) : Lott.Judgement
+
+end Lott.DSL
