Lott/Data/List.lean
@@ -1,4 +1,29 @@
-theorem List.map_singleton_join (xs : List α) : (xs.map fun x => [f x]).join = xs.map f :=
+namespace List
+
+theorem map_singleton_join (xs : List α) : (xs.map fun x => [f x]).join = xs.map f :=
   match xs with
   | [] => rfl
   | x :: xs' => by rw [List.map, List.map, List.join, List.singleton_append, xs'.map_singleton_join]
+
+theorem exists_gt (xs : List Nat)
+  : ∃ n : Nat, ∀ m : Nat, m ∈ xs → m < n := match xs with
+  | [] => .intro 0 fun x' x'in => nomatch x'in
+  | x :: xs' =>
+    let ⟨nxs', nxs'gt⟩ := xs'.exists_gt
+    let n := max (x + 1) nxs'
+    .intro n fun x' x'inxs => match List.mem_cons.mp x'inxs with
+      | .inl h => by
+        rw [h]
+        dsimp only [n]
+        rw [Nat.max_def]
+        split
+        · case isTrue h => exact Nat.lt_of_succ_le h
+        · case isFalse h => exact Nat.lt_succ_self _
+      | .inr x'inxs' =>
+        Nat.lt_of_lt_of_le (nxs'gt x' x'inxs') <| Nat.le_max_right _ _
+
+theorem exists_fresh (xs : List Nat) : ∃ n, n ∉ xs :=
+  let ⟨nxs, nxsgt⟩ := xs.exists_gt
+  .intro nxs fun nxsinxs => Nat.not_le_of_lt (nxsgt _ nxsinxs) <| Nat.le_refl _
+
+end List
