README.md
@@ -4,4 +4,5 @@ An [ott](https://github.com/ott-lang/ott)-like DSL embedded in Lean. Currently a
 
 ## References
 
-- Sewell, Peter, et al. "Ott: Effective tool support for the working semanticist." Journal of functional programming 20.1 (2010): 71-122.
+- Peter Sewell, Francesco Zappa Nardelli, Scott Owens, Gilles Peskine, Thomas Ridge, Susmit Sarkar, and others. 2010. Ott: Effective tool support for the working semanticist. Journal of functional programming 20, 1 (2010), 71–122.
+- Arthur Charguéraud. 2012. The locally nameless representation. Journal of automated reasoning 49, (2012), 363–408.
